Implement changes in semantics

FO-proof-systems/Formulas.thy
@@ -7,15 +7,13 @@ begin
 (* unrelated, but I need this in too many places. *)
 notation insert ("_ \<triangleright> _" [56,55] 55)
 
-datatype (atoms: 'p, vars: 'v, types: 'ty) formula = 
-    Atom 'p
-  | Bot                                                     ("\<bottom>")  
-  | Not "('p, 'v, 'ty) formula"                             ("\<^bold>\<not>")
-  | And "('p, 'v, 'ty) formula" "('p, 'v, 'ty) formula"     (infix "\<^bold>\<and>" 68)
-  | Or "('p, 'v, 'ty) formula" "('p, 'v, 'ty) formula"      (infix "\<^bold>\<or>" 68)
-  | Imp "('p, 'v, 'ty) formula" "('p, 'v, 'ty) formula"     (infixr "\<^bold>\<rightarrow>" 68)
-  | Exists 'ty 'v "('p, 'v, 'ty) formula"                   ("\<^bold>\<exists>\<^sub>_ _. _ " 0)
-  | All 'ty 'v "('p, 'v, 'ty) formula"                      ("\<^bold>\<forall>\<^sub>_ _. _" 0)
+datatype (atoms: 'a) formula = 
+    Atom 'a
+  | Bot                              ("\<bottom>")  
+  | Not "'a formula"                 ("\<^bold>\<not>")
+  | And "'a formula" "'a formula"    (infix "\<^bold>\<and>" 68)
+  | Or "'a formula" "'a formula"     (infix "\<^bold>\<or>" 68)
+  | Imp "'a formula" "'a formula"    (infixr "\<^bold>\<rightarrow>" 68)
 (* In a standard Isabelle/jEdit config, bold can be done with C-e rightarrow.
    I learned that way too late. *)
 (* I'm not sure I'm happy about the definition of what is an atom.
@@ -31,9 +29,7 @@ primrec subformulae where
 "subformulae (Not F) = Not F # subformulae F" |
 "subformulae (And F G) = And F G # subformulae F @ subformulae G" |
 "subformulae (Imp F G) = Imp F G # subformulae F @ subformulae G" |
-"subformulae (Or F G) = Or F G # subformulae F @ subformulae G" |
-"subformulae (Exists t x F) = (Exists t x F) # subformulae F" |
-"subformulae (All t x F) = (All t x F) # subformulae F"
+"subformulae (Or F G) = Or F G # subformulae F @ subformulae G"
 
 lemma atoms_are_subformulae: "Atom ` atoms F \<subseteq> set (subformulae F)"
   by (induction F) auto
@@ -62,85 +58,235 @@ definition Top ("\<top>") where
 "\<top> \<equiv> \<bottom> \<^bold>\<rightarrow> \<bottom>"
 lemma top_atoms_simp[simp]: "atoms \<top> = {}" unfolding Top_def by simp
 
-primrec BigAnd :: "('p, 'v, 'ty) formula list \<Rightarrow> ('p, 'v, 'ty) formula" ("\<^bold>\<And>_") where
+primrec BigAnd :: "'a formula list \<Rightarrow> 'a formula" ("\<^bold>\<And>_") where
 "\<^bold>\<And>Nil = (\<^bold>\<not>\<bottom>)" \<comment> \<open>essentially, it doesn't matter what I use here. But since I want to use this in CNFs, implication is not a nice thing to have.\<close> |
 "\<^bold>\<And>(F#Fs) = F \<^bold>\<and> \<^bold>\<And>Fs"
 
 lemma atoms_BigAnd[simp]: "atoms (\<^bold>\<And>Fs) = \<Union>(atoms ` set Fs)"
   by(induction Fs; simp)
 
-primrec BigOr :: "('p, 'v, 'ty) formula list \<Rightarrow> ('p, 'v, 'ty) formula" ("\<^bold>\<Or>_") where
+primrec BigOr :: "'a formula list \<Rightarrow> 'a formula" ("\<^bold>\<Or>_") where
 "\<^bold>\<Or>Nil = \<bottom>" |
 "\<^bold>\<Or>(F#Fs) = F \<^bold>\<or> \<^bold>\<Or>Fs"
+
+lemma atoms_BigOr[simp]: "atoms (\<^bold>\<Or>Fs) = \<Union>(atoms ` set Fs)"
+  by(induction Fs; simp)
 
 
 locale formula_syntax =
   fixes subst ::"'v \<Rightarrow> 'c \<Rightarrow> 'p \<Rightarrow> 'p"
     and vars  ::"'p \<Rightarrow> 'v set"
     and objs  ::"'p \<Rightarrow> 'c set"
-  assumes subst_subst_all: "v \<notin> vars (subst v c p)"
+    and dom   ::"'t \<Rightarrow> 'c list"
+  assumes subst_subst_all: "v \<notin> vars (subst v c p)" and
+          subst_replaces: "v \<in> vars p \<Longrightarrow> c \<in> objs (subst v c p)"
 begin
-  fun fsubst::"'v \<Rightarrow> 'c \<Rightarrow> ('p, 'v, 'ty) formula \<Rightarrow> ('p, 'v, 'ty) formula" where
+  fun fsubst::"'v \<Rightarrow> 'c \<Rightarrow> 'p formula \<Rightarrow> 'p formula" where
     "fsubst v c (Atom p) = Atom (subst v c p)" |
     "fsubst _ _ \<bottom> = \<bottom>" |
     "fsubst v c (Not \<phi>\<^sub>1) = Not (fsubst v c \<phi>\<^sub>1)" |
     "fsubst v c (And \<phi>\<^sub>1 \<phi>\<^sub>2) = And (fsubst v c \<phi>\<^sub>1) (fsubst v c \<phi>\<^sub>2)" |
     "fsubst v c (Or \<phi>\<^sub>1 \<phi>\<^sub>2) = Or (fsubst v c \<phi>\<^sub>1) (fsubst v c \<phi>\<^sub>2)" |
-    "fsubst v c (Imp \<phi>\<^sub>1 \<phi>\<^sub>2) = Imp (fsubst v c \<phi>\<^sub>1) (fsubst v c \<phi>\<^sub>2)" |
-    "fsubst v c (Exists t x \<phi>\<^sub>1) = (if x = v then Exists t x \<phi>\<^sub>1 else Exists t x (fsubst v c \<phi>\<^sub>1))" |
-    "fsubst v c (All t x \<phi>\<^sub>1) = (if x = v then All t x \<phi>\<^sub>1 else All t x (fsubst v c \<phi>\<^sub>1))"
+    "fsubst v c (Imp \<phi>\<^sub>1 \<phi>\<^sub>2) = Imp (fsubst v c \<phi>\<^sub>1) (fsubst v c \<phi>\<^sub>2)"
 
   
-  fun fvars::"('p, 'v, 'ty) formula \<Rightarrow> 'v set" where
+  fun fvars::"'p formula \<Rightarrow> 'v set" where
     "fvars (Atom p) = vars p" 
   | "fvars Bot = {}"
   | "fvars (Not \<phi>\<^sub>1) = fvars \<phi>\<^sub>1"
   | "fvars (And \<phi>\<^sub>1 \<phi>\<^sub>2) = fvars \<phi>\<^sub>1 \<union> fvars \<phi>\<^sub>2"
   | "fvars (Or \<phi>\<^sub>1 \<phi>\<^sub>2) = fvars \<phi>\<^sub>1 \<union> fvars \<phi>\<^sub>2"
   | "fvars (Imp \<phi>\<^sub>1 \<phi>\<^sub>2) = fvars \<phi>\<^sub>1 \<union> fvars \<phi>\<^sub>2"
-  | "fvars (Exists t x \<phi>) = fvars \<phi>"
-  | "fvars (All t x \<phi>) = fvars \<phi>"   
   
   
-  fun fobjs::"('p, 'v, 'ty) formula \<Rightarrow> 'c set" where
+  fun fobjs::"'p formula \<Rightarrow> 'c set" where
     "fobjs (Atom p) = objs p" 
   | "fobjs Bot = {}"
   | "fobjs (Not \<phi>\<^sub>1) = fobjs \<phi>\<^sub>1"
   | "fobjs (And \<phi>\<^sub>1 \<phi>\<^sub>2) = fobjs \<phi>\<^sub>1 \<union> fobjs \<phi>\<^sub>2"
   | "fobjs (Or \<phi>\<^sub>1 \<phi>\<^sub>2) = fobjs \<phi>\<^sub>1 \<union> fobjs \<phi>\<^sub>2"
   | "fobjs (Imp \<phi>\<^sub>1 \<phi>\<^sub>2) = fobjs \<phi>\<^sub>1 \<union> fobjs \<phi>\<^sub>2"
-  | "fobjs (Exists t x \<phi>) = fobjs \<phi>"
-  | "fobjs (All t x \<phi>) = fobjs \<phi>"   
-  
-  fun free_vars::"('p, 'v, 'ty) formula \<Rightarrow> 'v set" where
-    "free_vars (Atom p) = vars p" 
-  | "free_vars Bot = {}"
-  | "free_vars (Not \<phi>\<^sub>1) = free_vars \<phi>\<^sub>1"
-  | "free_vars (And \<phi>\<^sub>1 \<phi>\<^sub>2) = free_vars \<phi>\<^sub>1 \<union> free_vars \<phi>\<^sub>2"
-  | "free_vars (Or \<phi>\<^sub>1 \<phi>\<^sub>2) = free_vars \<phi>\<^sub>1 \<union> free_vars \<phi>\<^sub>2"
-  | "free_vars (Imp \<phi>\<^sub>1 \<phi>\<^sub>2) = free_vars \<phi>\<^sub>1 \<union> free_vars \<phi>\<^sub>2"
-  | "free_vars (Exists t x \<phi>\<^sub>1) = free_vars \<phi>\<^sub>1 - {x}"
-  | "free_vars (All t x \<phi>\<^sub>1) = free_vars \<phi>\<^sub>1 - {x}"
-  
-  (* these are not bound variables in the typical sense, but those that exist as bound variables
-      somewhere down the syntax tree *)
-  fun bound_vars::"('p, 'v, 'ty) formula \<Rightarrow> 'v set" where
-    "bound_vars (Atom p) = {}"
-  | "bound_vars Bot = {}"
-  | "bound_vars (Not \<phi>\<^sub>1) = bound_vars \<phi>\<^sub>1"
-  | "bound_vars (And \<phi>\<^sub>1 \<phi>\<^sub>2) = bound_vars \<phi>\<^sub>1 \<union> bound_vars \<phi>\<^sub>2"
-  | "bound_vars (Or \<phi>\<^sub>1 \<phi>\<^sub>2) = bound_vars \<phi>\<^sub>1 \<union> bound_vars \<phi>\<^sub>2"
-  | "bound_vars (Imp \<phi>\<^sub>1 \<phi>\<^sub>2) = bound_vars \<phi>\<^sub>1 \<union> bound_vars \<phi>\<^sub>2"
-  | "bound_vars (Exists t x \<phi>) = (free_vars \<phi> \<inter> {x}) \<union> bound_vars \<phi>"
-  | "bound_vars (All t x \<phi>) = (free_vars \<phi> \<inter> {x}) \<union> bound_vars \<phi>"
-  
-  lemma vars: "fvars \<phi> = free_vars \<phi> \<union> bound_vars \<phi>"
-    by (induction \<phi>) auto
-  
-  lemma fsubst_subst_free: "v \<notin> free_vars (fsubst v c f)"
-    by (induction f) (auto simp: subst_subst_all)
-  
-  lemma fsubst_leaves_bound: "v \<in> bound_vars f \<Longrightarrow> v \<in> bound_vars (fsubst v c f)"
-    by (induction f) auto
+
+  fun all::"'v \<Rightarrow> 't \<Rightarrow> 'p formula \<Rightarrow> 'p formula" ("\<^bold>\<forall>_ - _. _") where
+    "all v t \<phi> = \<^bold>\<And>(map (\<lambda>c. fsubst v c \<phi>) (dom t))"
+
+  fun exists::"'v \<Rightarrow> 't \<Rightarrow> 'p formula \<Rightarrow> 'p formula" ("\<^bold>\<forall>_ - _. _") where
+    "exists v t \<phi> = \<^bold>\<And>(map (\<lambda>c. fsubst v c \<phi>) (dom t))"
 end
+
+text\<open>Formulas are countable if their atoms are, and @{method countable_datatype} is really helpful with that.\<close> 
+instance formula :: (countable) countable by countable_datatype
+
+definition "prod_unions A B \<equiv> case A of (a,b) \<Rightarrow> case B of (c,d) \<Rightarrow> (a \<union> c, b \<union> d)"
+primrec pn_atoms where
+"pn_atoms (Atom A) = ({A},{})" |
+"pn_atoms Bot = ({},{})" |
+"pn_atoms (Not F) = prod.swap (pn_atoms F)" |
+"pn_atoms (And F G) = prod_unions (pn_atoms F) (pn_atoms G)" |
+"pn_atoms (Or F G) = prod_unions (pn_atoms F) (pn_atoms G)" |
+"pn_atoms (Imp F G) = prod_unions (prod.swap (pn_atoms F)) (pn_atoms G)"
+lemma pn_atoms_atoms: "atoms F = fst (pn_atoms F) \<union> snd (pn_atoms F)"
+  by(induction F) (auto simp add: prod_unions_def split: prod.splits)
+
+text\<open>A very trivial simplifier.
+Does wonders as a postprocessor for the Harrison-style Craig interpolations.\<close>
+context begin
+definition "isstop F \<equiv> F = \<^bold>\<not>\<bottom> \<or> F = \<top>"
+fun simplify_consts where
+"simplify_consts (Atom k) = Atom k" |
+"simplify_consts \<bottom> = \<bottom>" |
+"simplify_consts (Not F) = (let S = simplify_consts F in case S of (Not G) \<Rightarrow> G | _ \<Rightarrow>
+  if isstop S then \<bottom> else \<^bold>\<not> S)" |
+"simplify_consts (And F G) = (let S = simplify_consts F; T = simplify_consts G in (
+  if S = \<bottom> then \<bottom> else
+  if isstop S then T \<comment> \<open>not \<open>\<top>\<close>, \<open>T\<close>\<close> else
+  if T = \<bottom> then \<bottom> else
+  if isstop T then S else
+  if S = T then S else
+  S \<^bold>\<and> T))" |
+"simplify_consts (Or F G) = (let S = simplify_consts F; T = simplify_consts G in (
+  if S = \<bottom> then T else
+  if isstop S then \<top> else
+  if T = \<bottom> then S else
+  if isstop T then \<top> else
+  if S = T then S else
+  S \<^bold>\<or> T))" |
+"simplify_consts (Imp F G) = (let S = simplify_consts F; T = simplify_consts G in (
+  if S = \<bottom> then \<top> else
+  if isstop S then T else
+  if isstop T then \<top> else
+  if T = \<bottom> then \<^bold>\<not> S else
+  if S = T then \<top> else
+  case S of Not H \<Rightarrow> (case T of Not I \<Rightarrow> 
+    I \<^bold>\<rightarrow> H | _ \<Rightarrow> 
+    H \<^bold>\<or> T) | _ \<Rightarrow>
+    S \<^bold>\<rightarrow> T))"
+
+lemma simplify_consts_size_le: "size (simplify_consts F) \<le> size F"
+proof -
+  have [simp]: "Suc (Suc 0) \<le> size F + size G" for F G :: "'a formula" by(cases F; cases G; simp)
+  show ?thesis by(induction F; fastforce simp add: Let_def isstop_def Top_def split: formula.splits)
+qed
+
+lemma simplify_const: "atoms F = {} \<Longrightarrow> isstop (simplify_consts F) \<or> (simplify_consts F) = \<bottom>"
+  by(induction F; fastforce simp add: Let_def isstop_def Top_def split: formula.splits)
+value "(size \<top>, size (\<^bold>\<not>\<bottom>))" (* this is why I need isstop in this lemma and can't write simplify_consts
+  in a way that this lemma can say \<in> {\<top>, \<bottom>} *)
+
+end
+  
+(*
+Here's a useful little function for testing a conjecture on "a few" examples: 
+*)
+fun all_formulas_of_size where
+"all_formulas_of_size K 0 = {\<bottom>} \<union> Atom ` K" |
+"all_formulas_of_size K (Suc n) = (
+  let af = \<Union>(set [all_formulas_of_size K m. m \<leftarrow> [0..<Suc n]]) in
+  (\<Union>F\<in>af.
+    (\<Union>G\<in>af. if size F + size G \<le> Suc n then {And F G, Or F G, Imp F G} else {}) 
+   \<union> (if size F \<le> Suc n then {Not F} else {})) 
+  \<union> af)"
+(* this set obviously grows exponentially (with a base of 5 approximately).
+   size 7 produces 26032 formulas, which is probably the last value
+   where I can test anything meaningfully with this implementation. *)
+
+lemma all_formulas_of_size: "F \<in> all_formulas_of_size K n \<longleftrightarrow> (size F \<le> Suc n \<and> atoms F \<subseteq> K)" (is "?l \<longleftrightarrow> ?r")
+proof -
+  have rl: "?r \<Longrightarrow> ?l"
+  proof(induction F arbitrary: n)
+    case (Atom x)
+    have *: "Atom x \<in> all_formulas_of_size K 0" using Atom by simp
+    hence **: "Atom x \<in> \<Union> (all_formulas_of_size K ` set [0..<Suc m])" for m
+      by (simp; metis atLeastLessThan_iff le_zero_eq not_le)
+    thus ?case using Atom by(cases n; simp)
+  next
+    case Bot
+    have *: "Bot \<in> all_formulas_of_size K 0" by simp
+    hence **: "Bot \<in> \<Union> (all_formulas_of_size K ` set [0..<Suc m])" for m
+      by (simp; metis atLeastLessThan_iff le_zero_eq not_le)
+    then show ?case using Bot by(cases n; simp)
+  next
+    case (Not F)
+    have *: "size F \<le> n" using Not by simp
+    then obtain m where n[simp]: "n = Suc m" by (metis Suc_diff_1 formula.size_neq leD neq0_conv)
+    with Not have IH: "F \<in> all_formulas_of_size K m" by simp
+    then show ?case using * by(simp add: bexI[where x=F])
+  next
+    case (And F G)
+    with And have *: "size F + size G \<le> n" by simp
+    then obtain m where n[simp]: "n = Suc m"
+      by (metis Suc_diff_1 add_is_0 formula.size_neq le_zero_eq neq0_conv)
+    then obtain nF nG where nFG[simp]: "size F \<le> nF" "size G \<le> nG" "n = nF + nG"
+      by (metis * add.assoc nat_le_iff_add order_refl)
+    then obtain mF mG where mFG[simp]: "nF = Suc mF" "nG = Suc mG"
+      by (metis Suc_diff_1 formula.size_neq leD neq0_conv)
+    with And have IH: "F \<in> all_formulas_of_size K mF" "G \<in> all_formulas_of_size K mG" 
+      using nFG by simp+
+    let ?af = "\<Union>(set [all_formulas_of_size K m. m \<leftarrow> [0..<Suc m]])"
+    have r: "F \<in> all_formulas_of_size K mF \<Longrightarrow> mF \<le> n \<Longrightarrow> F \<in> \<Union>(set (map (all_formulas_of_size K) [0..<Suc n]))"
+      for F mF n by fastforce
+    have af: "F \<in> ?af" "G \<in> ?af" using nFG(3) by(intro IH[THEN r]; simp)+
+    have m: "F \<^bold>\<and> G \<in> (if size F + size G \<le> Suc m then {F \<^bold>\<and> G, F \<^bold>\<or> G, F \<^bold>\<rightarrow> G} else {})" using * by simp
+    from IH * show ?case using af by(simp only: n all_formulas_of_size.simps Let_def, insert m) fast
+  next
+    case (Or F G) case (Imp F G) \<comment> \<open>analogous\<close> (*<*)
+  next
+    case (Or F G)
+    with Or have *: "size F + size G \<le> n" by simp
+    then obtain m where n[simp]: "n = Suc m"
+      by (metis Suc_diff_1 add_is_0 formula.size_neq le_zero_eq neq0_conv)
+    then obtain nF nG where nFG[simp]: "size F \<le> nF" "size G \<le> nG" "n = nF + nG"
+      by (metis * add.assoc nat_le_iff_add order_refl)
+    then obtain mF mG where mFG[simp]: "nF = Suc mF" "nG = Suc mG"
+      by (metis Suc_diff_1 formula.size_neq leD neq0_conv)
+    with Or have IH: "F \<in> all_formulas_of_size K mF" "G \<in> all_formulas_of_size K mG" 
+      using nFG by simp+
+    let ?af = "\<Union>(set [all_formulas_of_size K m. m \<leftarrow> [0..<Suc m]])"
+    have r: "F \<in> all_formulas_of_size K mF \<Longrightarrow> mF \<le> n \<Longrightarrow> F \<in> \<Union>(set (map (all_formulas_of_size K) [0..<Suc n]))"
+      for F mF n by fastforce
+    have af: "F \<in> ?af" "G \<in> ?af" using nFG(3) by(intro IH[THEN r]; simp)+
+    have m: "Or F G \<in> (if size F + size G \<le> Suc m then {F \<^bold>\<and> G, F \<^bold>\<or> G, F \<^bold>\<rightarrow> G} else {})" using * by simp
+    from IH * show ?case using af by(simp only: n all_formulas_of_size.simps Let_def, insert m) fast
+  next
+    case (Imp F G)
+    with Imp have *: "size F + size G \<le> n" by simp
+    then obtain m where n[simp]: "n = Suc m"
+      by (metis Suc_diff_1 add_is_0 formula.size_neq le_zero_eq neq0_conv)
+    then obtain nF nG where nFG[simp]: "size F \<le> nF" "size G \<le> nG" "n = nF + nG"
+      by (metis * add.assoc nat_le_iff_add order_refl)
+    then obtain mF mG where mFG[simp]: "nF = Suc mF" "nG = Suc mG"
+      by (metis Suc_diff_1 formula.size_neq leD neq0_conv)
+    with Imp have IH: "F \<in> all_formulas_of_size K mF" "G \<in> all_formulas_of_size K mG" 
+      using nFG by simp+
+    let ?af = "\<Union>(set [all_formulas_of_size K m. m \<leftarrow> [0..<Suc m]])"
+    have r: "F \<in> all_formulas_of_size K mF \<Longrightarrow> mF \<le> n \<Longrightarrow> F \<in> \<Union>(set (map (all_formulas_of_size K) [0..<Suc n]))"
+      for F mF n by fastforce
+    have af: "F \<in> ?af" "G \<in> ?af" using nFG(3) by(intro IH[THEN r]; simp)+
+    have m: "Imp F G \<in> (if size F + size G \<le> Suc m then {F \<^bold>\<and> G, F \<^bold>\<or> G, F \<^bold>\<rightarrow> G} else {})" using * by simp
+    from IH * show ?case using af by(simp only: n all_formulas_of_size.simps Let_def, insert m) fast
+  (*>*)
+  qed
+  have lr: ?r if l: ?l 
+  proof
+    have *: "F \<in> all_formulas_of_size K x \<Longrightarrow> F \<in> all_formulas_of_size K (x + n)" for x n
+      by(induction n; simp)
+    show "size F \<le> Suc n" using l
+      by(induction n; auto split: if_splits) (metis "*" le_SucI le_eq_less_or_eq le_iff_add)
+    show "atoms F \<subseteq> K" using l
+      proof(induction n arbitrary: F rule: less_induct)
+        case (less x)
+        then show ?case proof(cases x)
+          case 0 with less show ?thesis by force
+        next
+          case (Suc y) with less show ?thesis 
+            by(simp only: all_formulas_of_size.simps Let_def) (fastforce simp add: less_Suc_eq split: if_splits)
+        qed
+      qed
+  qed
+  from lr rl show ?thesis proof qed
+qed
+(* At first I thought: why would I prove anything about all_formulas_of_size, I only want to test a conjecture with it.
+   Guess why: it was broken.
+   Granted, I spent too much time on this. *)
+
 end
