FO-proof-systems/Sema.thy
@@ -6,64 +6,141 @@ begin
 type_synonym 'a valuation = "'a \<Rightarrow> bool"
 text\<open>The implicit statement here is that an assignment or valuation is always defined on all atoms (because HOL is a total logic).
 Thus, there are no unsuitable assignments.\<close>
-      
-locale formula_semantics = formula_syntax subst vars objs
-  for subst::"'v \<Rightarrow> 'c \<Rightarrow> 'p \<Rightarrow> 'p"
-  and vars ::"'p \<Rightarrow> 'v set"
-  and objs ::"'p \<Rightarrow> 'c set"
-  +
-  fixes dom::"'ty \<Rightarrow> 'c list"
-begin
-                                               
-fun height::"('p valuation \<times> ('p, 'v, 'ty) formula) \<Rightarrow> nat" where
-"height (v, (Atom _)) = 0" |
-"height (v, \<bottom>) = 0" |
-"height (v, (Not \<phi>)) = 1 + height (v, \<phi>)" |
-"height (v, (And \<phi>\<^sub>1 \<phi>\<^sub>2)) = 1 + max (height (v, \<phi>\<^sub>1)) (height (v, \<phi>\<^sub>2))" |
-"height (v, (Or \<phi>\<^sub>1 \<phi>\<^sub>2)) = 1 + max (height (v, \<phi>\<^sub>1)) (height (v, \<phi>\<^sub>2))" |
-"height (v, (Imp \<phi>\<^sub>1 \<phi>\<^sub>2)) = 1 + max (height (v, \<phi>\<^sub>1)) (height (v, \<phi>\<^sub>2))" |
-"height (v, (Exists t x \<phi>\<^sub>1)) = 1 + height (v, \<phi>\<^sub>1)" |
-"height (v, (All t x \<phi>\<^sub>1)) = 1 + height (v, \<phi>\<^sub>1)"
 
-lemma fsubst_maintains_height: "height (v, f) = height (v, fsubst x x1 f)"
-  by (induction f) auto
-
-function formula_semantics :: "'p valuation \<Rightarrow> ('p, 'v, 'ty) formula \<Rightarrow> bool" (infix "\<Turnstile>" 61) where
+primrec formula_semantics :: "'a valuation \<Rightarrow> 'a formula \<Rightarrow> bool" (infix "\<Turnstile>" 51) where
 "\<A> \<Turnstile> Atom k = \<A> k" |
 "_ \<Turnstile> \<bottom> = False" |
-"\<A> \<Turnstile> Not \<phi> = (\<not> \<A> \<Turnstile> \<phi>)" |
-"\<A> \<Turnstile> And \<phi>\<^sub>1 \<phi>\<^sub>2 = (\<A> \<Turnstile> \<phi>\<^sub>1 \<and> \<A> \<Turnstile> \<phi>\<^sub>2)" |
-"\<A> \<Turnstile> Or \<phi>\<^sub>1 \<phi>\<^sub>2 = (\<A> \<Turnstile> \<phi>\<^sub>1 \<or> \<A> \<Turnstile> \<phi>\<^sub>2)" |
-"\<A> \<Turnstile> Imp \<phi>\<^sub>1 \<phi>\<^sub>2 = (\<A> \<Turnstile> \<phi>\<^sub>1 \<longrightarrow> \<A> \<Turnstile> \<phi>\<^sub>2)" |
-"\<A> \<Turnstile> Exists t x \<phi>\<^sub>1 = (find (\<lambda>v. \<A> \<Turnstile> (fsubst x v \<phi>\<^sub>1)) (dom t) \<noteq> None)" |
-"\<A> \<Turnstile> All t x \<phi>\<^sub>1 = (list_all (\<lambda>v. \<A> \<Turnstile> (fsubst x v \<phi>\<^sub>1)) (dom t))"
-  by (pat_completeness) auto
-termination formula_semantics
-  by (relation "measure height")(auto simp add: sym[OF fsubst_maintains_height])
+"\<A> \<Turnstile> Not F = (\<not> \<A> \<Turnstile> F)" |
+"\<A> \<Turnstile> And F G = (\<A> \<Turnstile> F \<and> \<A> \<Turnstile> G)" |
+"\<A> \<Turnstile> Or F G = (\<A> \<Turnstile> F \<or> \<A> \<Turnstile> G)" |
+"\<A> \<Turnstile> Imp F G = (\<A> \<Turnstile> F \<longrightarrow> \<A> \<Turnstile> G)"
 
 abbreviation valid ("\<Turnstile> _" 51) where
 "\<Turnstile> F \<equiv> \<forall>A. A \<Turnstile> F"
 
-definition formula_entailment :: "('p, 'v, 'ty) formula set \<Rightarrow> ('p, 'v, 'ty) formula \<Rightarrow> bool" 
-  (infix "\<TTurnstile>" 63) where
-"\<Gamma> \<TTurnstile> F \<equiv> (\<forall>\<A>. ((\<forall>G \<in> \<Gamma>. \<A> \<Turnstile> G) \<longrightarrow> (\<A> \<Turnstile> F)))"
-
 lemma irrelevant_atom[simp]: "A \<notin> atoms F \<Longrightarrow> (\<A>(A := V)) \<Turnstile> F \<longleftrightarrow> \<A> \<Turnstile> F"
-  by (induction F; auto)
+  by (induction F; simp)
 lemma relevant_atoms_same_semantics: "\<forall>k \<in> atoms F. \<A>\<^sub>1 k = \<A>\<^sub>2 k \<Longrightarrow> \<A>\<^sub>1 \<Turnstile> F \<longleftrightarrow> \<A>\<^sub>2 \<Turnstile> F"
   by(induction F; simp)
 
+context begin
+text\<open>Just a definition more similar to~\<^cite>\<open>\<open>p. 5\<close> in "schoening1987logik"\<close>.
+Unfortunately, using this as the main definition would get in the way of automated reasoning all the time.\<close>
+private primrec formula_semantics_alt where
+"formula_semantics_alt \<A> (Atom k) = \<A> k" |
+"formula_semantics_alt \<A> (Bot) = False" |
+"formula_semantics_alt \<A> (Not a) = (if formula_semantics_alt \<A> a then False else True)" |
+"formula_semantics_alt \<A> (And a b) = (if formula_semantics_alt \<A> a then formula_semantics_alt \<A> b else False)" |
+"formula_semantics_alt \<A> (Or a b) = (if formula_semantics_alt \<A> a then True else formula_semantics_alt \<A> b)" |
+"formula_semantics_alt \<A> (Imp a b) = (if formula_semantics_alt \<A> a then formula_semantics_alt \<A> b else True)"
+private lemma "formula_semantics_alt \<A> F \<longleftrightarrow> \<A> \<Turnstile> F"
+  by(induction F; simp)
+
+text\<open>If you fancy a definition more similar to~\<^cite>\<open>\<open>p. 39\<close> in "gallier2015logic"\<close>,
+this is probably the closest you can go without going incredibly ugly.\<close>
+private primrec formula_semantics_tt where
+"formula_semantics_tt \<A> (Atom k) = \<A> k" |
+"formula_semantics_tt \<A> (Bot) = False" |
+"formula_semantics_tt \<A> (Not a) = (case formula_semantics_tt \<A> a of True \<Rightarrow> False | False \<Rightarrow> True)" |
+"formula_semantics_tt \<A> (And a b) = (case (formula_semantics_tt \<A> a, formula_semantics_tt \<A> b) of
+  (False, False) \<Rightarrow> False
+| (False, True) \<Rightarrow> False
+| (True, False) \<Rightarrow> False
+| (True, True) \<Rightarrow> True)" |
+"formula_semantics_tt \<A> (Or a b) = (case (formula_semantics_tt \<A> a, formula_semantics_tt \<A> b) of
+  (False, False) \<Rightarrow> False
+| (False, True) \<Rightarrow> True
+| (True, False) \<Rightarrow> True
+| (True, True) \<Rightarrow> True)" |
+"formula_semantics_tt \<A> (Imp a b) = (case (formula_semantics_tt \<A> a, formula_semantics_tt \<A> b) of
+  (False, False) \<Rightarrow> True
+| (False, True) \<Rightarrow> True
+| (True, False) \<Rightarrow> False
+| (True, True) \<Rightarrow> True)"
+private lemma "A \<Turnstile> F \<longleftrightarrow> formula_semantics_tt A F"
+  by(induction F; simp split: prod.splits bool.splits)
+end
+
+definition entailment :: "'a formula set \<Rightarrow> 'a formula \<Rightarrow> bool" ("(_ \<TTurnstile>/ _)" (* \TTurnstile *) [53,53] 53) where
+"\<Gamma> \<TTurnstile> F \<equiv> (\<forall>\<A>. ((\<forall>G \<in> \<Gamma>. \<A> \<Turnstile> G) \<longrightarrow> (\<A> \<Turnstile> F)))"
+text\<open>We write entailment differently than semantics (\<open>\<Turnstile>\<close> vs. \<open>\<TTurnstile>\<close>).
+For humans, it is usually pretty clear what is meant in a specific situation, 
+but it often needs to be decided from context that Isabelle/HOL does not have.\<close>
+  
+text\<open>Some helpers for the derived connectives\<close>
 lemma top_semantics[simp,intro!]: "A \<Turnstile> \<top>" unfolding Top_def by simp
 lemma BigAnd_semantics[simp]: "A \<Turnstile> \<^bold>\<And>F \<longleftrightarrow> (\<forall>f \<in> set F. A \<Turnstile> f)" by(induction F; simp)
 lemma BigOr_semantics[simp]: "A \<Turnstile> \<^bold>\<Or>F \<longleftrightarrow> (\<exists>f \<in> set F. A \<Turnstile> f)" by(induction F; simp)
     
+text\<open>Definitions for sets of formulae, used for compactness and model existence.\<close>
 
 definition "sat S \<equiv> \<exists>\<A>. \<forall>F \<in> S. \<A> \<Turnstile> F"
 definition "fin_sat S \<equiv> (\<forall>s \<subseteq> S. finite s \<longrightarrow> sat s)"
   
 lemma entail_sat: "\<Gamma> \<TTurnstile> \<bottom> \<longleftrightarrow> \<not> sat \<Gamma>" (* btw. *)
-  unfolding sat_def formula_entailment_def by simp
+  unfolding sat_def entailment_def by simp
 
-end
-
+lemma pn_atoms_updates: "p \<notin> snd (pn_atoms F) \<Longrightarrow> n \<notin> fst (pn_atoms F) \<Longrightarrow>
+  ((M \<Turnstile> F \<longrightarrow> (M(p := True) \<Turnstile> F \<and> M(n := False) \<Turnstile> F))) \<and> ((\<not>(M \<Turnstile> F)) \<longrightarrow> \<not>(M(n := True) \<Turnstile> F) \<and> \<not>(M(p := False) \<Turnstile> F))"
+proof(induction F arbitrary: n p)
+  case (Imp F G)
+  from Imp.prems have prems:
+     "p \<notin> fst (pn_atoms F)" "p \<notin> snd (pn_atoms G)"
+     "n \<notin> snd (pn_atoms F)" "n \<notin> fst (pn_atoms G)"
+    by(simp_all add: prod_unions_def split: prod.splits)
+  have IH1: "M \<Turnstile> F \<Longrightarrow> M(n := True) \<Turnstile> F" " M \<Turnstile> F \<Longrightarrow> M(p := False) \<Turnstile> F" "\<not> M \<Turnstile> F \<Longrightarrow> \<not> M(p := True) \<Turnstile> F" "\<not> M \<Turnstile> F \<Longrightarrow> \<not> M(n := False) \<Turnstile> F"
+    using Imp.IH(1)[OF prems(3) prems(1)] by blast+
+  have IH2: "M \<Turnstile> G \<Longrightarrow> M(p := True) \<Turnstile> G" "M \<Turnstile> G \<Longrightarrow> M(n := False) \<Turnstile> G" "\<not> M \<Turnstile> G \<Longrightarrow> \<not> M(n := True) \<Turnstile> G" "\<not> M \<Turnstile> G \<Longrightarrow> \<not> M(p := False) \<Turnstile> G" 
+    using Imp.IH(2)[OF prems(2) prems(4)] by blast+
+   show ?case proof(intro conjI; intro impI)
+     assume "M \<Turnstile> F \<^bold>\<rightarrow> G"
+     then consider "\<not> M \<Turnstile> F" | "M \<Turnstile>G" by auto
+     thus "M(p := True) \<Turnstile> F \<^bold>\<rightarrow> G \<and> M(n := False) \<Turnstile> F \<^bold>\<rightarrow> G" using IH1(3,4) IH2(1,2) by cases simp_all
+   next
+     assume "\<not>(M \<Turnstile> F \<^bold>\<rightarrow> G)"
+     hence "M \<Turnstile> F" "\<not>M \<Turnstile> G" by simp_all
+     thus "\<not> M(n := True) \<Turnstile> F \<^bold>\<rightarrow> G \<and> \<not> M(p := False) \<Turnstile> F \<^bold>\<rightarrow> G" using IH1(1,2) IH2(3,4) by simp
+   qed
+ next
+  case (And F G)
+  from And.prems have prems:
+     "p \<notin> snd (pn_atoms F)" "p \<notin> snd (pn_atoms G)"
+     "n \<notin> fst (pn_atoms F)" "n \<notin> fst (pn_atoms G)"
+    by(simp_all add: prod_unions_def split: prod.splits)
+  have IH1: "M \<Turnstile> F \<Longrightarrow> M(p := True) \<Turnstile> F" " M \<Turnstile> F \<Longrightarrow> M(n := False) \<Turnstile> F" "\<not> M \<Turnstile> F \<Longrightarrow> \<not> M(n := True) \<Turnstile> F" "\<not> M \<Turnstile> F \<Longrightarrow> \<not> M(p := False) \<Turnstile> F"
+    using And.IH(1)[OF prems(1) prems(3)] by blast+
+  have IH2: "M \<Turnstile> G \<Longrightarrow> M(p := True) \<Turnstile> G" "M \<Turnstile> G \<Longrightarrow> M(n := False) \<Turnstile> G" "\<not> M \<Turnstile> G \<Longrightarrow> \<not> M(n := True) \<Turnstile> G" "\<not> M \<Turnstile> G \<Longrightarrow> \<not> M(p := False) \<Turnstile> G" 
+    using And.IH(2)[OF prems(2) prems(4)] by blast+
+  show ?case proof(intro conjI; intro impI)
+    assume "\<not>M \<Turnstile> F \<^bold>\<and> G"
+    then consider "\<not> M \<Turnstile> F" | "\<not> M \<Turnstile>G" by auto
+    thus "\<not> M(n := True) \<Turnstile> F \<^bold>\<and> G \<and> \<not> M(p := False) \<Turnstile> F \<^bold>\<and> G" using IH1 IH2 by cases simp_all
+  next
+    assume "M \<Turnstile> F \<^bold>\<and> G"
+    hence "M \<Turnstile> F" "M \<Turnstile> G" by simp_all
+    thus "M(p := True) \<Turnstile> F \<^bold>\<and> G \<and> M(n := False) \<Turnstile> F \<^bold>\<and> G " using IH1 IH2 by simp
+  qed
+next
+  case (Or F G)
+  from Or.prems have prems:
+     "p \<notin> snd (pn_atoms F)" "p \<notin> snd (pn_atoms G)"
+     "n \<notin> fst (pn_atoms F)" "n \<notin> fst (pn_atoms G)"
+    by(simp_all add: prod_unions_def split: prod.splits)
+  have IH1: "M \<Turnstile> F \<Longrightarrow> M(p := True) \<Turnstile> F" " M \<Turnstile> F \<Longrightarrow> M(n := False) \<Turnstile> F" "\<not> M \<Turnstile> F \<Longrightarrow> \<not> M(n := True) \<Turnstile> F" "\<not> M \<Turnstile> F \<Longrightarrow> \<not> M(p := False) \<Turnstile> F"
+    using Or.IH(1)[OF prems(1) prems(3)] by blast+
+  have IH2: "M \<Turnstile> G \<Longrightarrow> M(p := True) \<Turnstile> G" "M \<Turnstile> G \<Longrightarrow> M(n := False) \<Turnstile> G" "\<not> M \<Turnstile> G \<Longrightarrow> \<not> M(n := True) \<Turnstile> G" "\<not> M \<Turnstile> G \<Longrightarrow> \<not> M(p := False) \<Turnstile> G" 
+    using Or.IH(2)[OF prems(2) prems(4)] by blast+
+  show ?case proof(intro conjI; intro impI)
+    assume "M \<Turnstile> F \<^bold>\<or> G"
+    then consider "M \<Turnstile> F" | "M \<Turnstile>G" by auto
+    thus "M(p := True) \<Turnstile> F \<^bold>\<or> G \<and> M(n := False) \<Turnstile> F \<^bold>\<or> G" using IH1 IH2 by cases simp_all
+  next
+    assume "\<not>M \<Turnstile> F \<^bold>\<or> G"
+    hence "\<not>M \<Turnstile> F" "\<not>M \<Turnstile> G" by simp_all
+    thus "\<not>M(n := True) \<Turnstile> F \<^bold>\<or> G \<and> \<not>M(p := False) \<Turnstile> F \<^bold>\<or> G " using IH1 IH2 by simp
+  qed
+qed simp_all
+  
+lemma const_simplifier_correct: "\<A> \<Turnstile> simplify_consts F \<longleftrightarrow> \<A> \<Turnstile> F"
+  by (induction F) (auto simp add: Let_def isstop_def Top_def split: formula.splits) 
 end
