PDDL_STRIPS_Semantics.thy
@@ -72,9 +72,9 @@ datatype type = Either (primitives: "name list")
 
 text \<open>An effect contains a list of values to be added, and a list of values
   to be removed.\<close>
-datatype ('ent, 'var, 'ty) ast_effect = 
-  Effect  (adds: "(('ent atom, 'var, 'ty) formula) list") 
-          (dels: "(('ent atom, 'var, 'ty) formula) list")
+datatype 'ent ast_effect = 
+  Effect  (adds: "(('ent atom) formula) list") 
+          (dels: "(('ent atom) formula) list")
 
 text \<open>Variables are identified by their names.\<close>
 datatype variable = varname: Var name
@@ -82,19 +82,14 @@ text \<open>Objects and constants are identified by their names\<close>
 datatype object = name: Obj name
 
 datatype "term" = VAR variable | CONST object
-hide_const (open) VAR CONST \<comment> \<open>Refer to constructors by qualified names only\<close>
+hide_const (open) VAR CONST
 
-find_theorems name: "map*term"
 
-datatype inst_term = VAR variable | OBJ object
-hide_const (open) VAR OBJ
+type_synonym schematic_formula = "(term atom) formula"
+type_synonym schematic_effect = "term ast_effect"
 
-type_synonym schematic_formula = "(term atom, variable, type) formula"
-type_synonym schematic_effect = "(term, variable, type) ast_effect"
-
-(* should not be called ground, but instantiated *)
-type_synonym inst_formula = "(inst_term atom, variable, type) formula"
-type_synonym inst_effect = "(inst_term, variable, type) ast_effect"
+type_synonym ground_formula = "(object atom) formula"
+type_synonym ground_effect = "object ast_effect"
 
 subsubsection \<open>Domains\<close>
 
@@ -129,20 +124,19 @@ subsubsection \<open>Problems\<close>
 
 
 text \<open>A fact is a predicate applied to objects.\<close>
-text \<open>Changed to inst_term, because this makes some other changes easier.
+text \<open>Changed to object, because this makes some other changes easier.
     However, the change from object term to ground term in general requires
     us to assert that variables in instantiations are bound.\<close>
-text \<open> Question: are facts only using in effects? See \<open>wf_fact\<close> as well. \<close>
-type_synonym fact = "predicate \<times> inst_term list"
+text \<open> Question: are facts only used in effects? See \<open>wf_fact\<close> as well. \<close>
+type_synonym fact = "predicate \<times> object list"
 
 text \<open>A problem consists of a domain, a list of objects,
   a description of the initial state, and a description of the goal state. \<close>
 datatype ast_problem = Problem
   (domain: ast_domain)
   (objects: "(object \<times> type) list")
-  (init: "inst_formula list")
-  (goal: "inst_formula")
-
+  (init: "ground_formula list")
+  (goal: "schematic_formula")
 
 subsubsection \<open>Plans\<close>
 datatype plan_action = PAction
@@ -156,92 +150,74 @@ text \<open>The following datatype represents an action scheme that has been
   instantiated by replacing the arguments with concrete objects,
   also called ground action.
 \<close>
-datatype inst_action = Inst_Action
-  (precondition: "inst_formula")
-  (effect: "inst_effect")
+datatype ground_action = Ground_Action
+  (precondition: "ground_formula")
+  (effect: "ground_effect")
 
 (* Syntax helpers for schematic formulae *)
 
-fun schematic_term_subst::"variable \<Rightarrow> object \<Rightarrow> term \<Rightarrow> term" where
-  "schematic_term_subst v obj (term.VAR x) = (if (x = v) then (term.CONST obj) else term.VAR x)" 
-| "schematic_term_subst _ _ (term.CONST obj) = term.CONST obj"
+fun term_vars where
+  "term_vars (term.VAR x) = {x}" 
+| "term_vars (term.CONST c) = {}"
 
-abbreviation schematic_term_atom_subst where
-"schematic_term_atom_subst v obj \<equiv> map_atom (schematic_term_subst v obj)"
+fun term_objs where
+  "term_objs (term.VAR x) = {}"
+| "term_objs (term.CONST obj) = {obj}"
 
-fun schematic_term_vars where
-  "schematic_term_vars (term.VAR x) = {x}" 
-| "schematic_term_vars (term.CONST c) = {}"
+fun term_subst::"variable \<Rightarrow> object \<Rightarrow> term \<Rightarrow> term" where
+  "term_subst v obj (term.VAR x) = (if (x = v) then (term.CONST obj) else term.VAR x)" 
+| "term_subst _ _ (term.CONST obj) = term.CONST obj"
 
-definition schematic_term_atom_vars where
-"schematic_term_atom_vars \<equiv> \<Union> o ent o (map_atom schematic_term_vars)"
+abbreviation term_atom_subst where
+"term_atom_subst v obj \<equiv> map_atom (term_subst v obj)"
 
-fun schematic_term_objs where
-  "schematic_term_objs (term.VAR x) = {}"
-| "schematic_term_objs (term.CONST obj) = {obj}"
+definition term_atom_vars where
+"term_atom_vars \<equiv> \<Union> o ent o (map_atom term_vars)"
 
-definition schematic_term_atom_objs where
-"schematic_term_atom_objs \<equiv> \<Union> o ent o (map_atom schematic_term_objs)"
+definition term_atom_objs where
+"term_atom_objs \<equiv> \<Union> o ent o (map_atom term_objs)"
 
-lemma sa_subst_all: "v \<notin> schematic_term_atom_vars (schematic_term_atom_subst v obj a)"
+
+lemma tav_alt: "term_atom_vars x = \<Union> (term_vars ` ent x)" 
+  unfolding term_atom_vars_def by (simp add: atom.set_map) 
+
+lemma tao_alt: "term_atom_objs x = \<Union> (term_objs ` ent x)" 
+  unfolding term_atom_objs_def by (simp add: atom.set_map) 
+
+lemma tav_empty: "term_atom_vars x = {} \<longleftrightarrow> (\<forall>e \<in> ent x. term_vars e = {})"
+  using tav_alt by auto
+
+lemma tavm_alt: "term_atom_vars (map_atom f x) = \<Union> ((term_vars o f) ` ent x)"
+  unfolding term_atom_vars_def by (simp add: atom.map_comp atom.set_map)
+
+lemma taom_alt: "term_atom_objs (map_atom f x) = \<Union> ((term_objs o f) ` ent x)"
+  unfolding term_atom_objs_def by (simp add: atom.map_comp atom.set_map)
+
+lemma subst_subst_all: "v \<notin> term_atom_vars (term_atom_subst v obj a)"
 proof -
-  have "schematic_term_atom_vars (schematic_term_atom_subst v obj a) = (\<Union> o ent o (map_atom schematic_term_vars)) (map_atom (schematic_term_subst v obj) a)" unfolding schematic_term_atom_vars_def by simp
-  also have "...  = \<Union> (ent (map_atom schematic_term_vars (map_atom (schematic_term_subst v obj) a)))" by simp
-  also have "... = \<Union> (ent (map_atom (schematic_term_vars o (schematic_term_subst v obj)) a))" by (simp add: atom.map_comp)
+  have "term_atom_vars (term_atom_subst v obj a) = (\<Union> o ent o (map_atom term_vars)) (map_atom (term_subst v obj) a)" unfolding term_atom_vars_def by simp
+  also have "...  = \<Union> (ent (map_atom term_vars (map_atom (term_subst v obj) a)))" by simp
+  also have "... = \<Union> (ent (map_atom (term_vars o (term_subst v obj)) a))" by (simp add: atom.map_comp)
   finally 
-  have "schematic_term_atom_vars (schematic_term_atom_subst v obj a) = \<Union> ((schematic_term_vars o (schematic_term_subst v obj)) ` ent a)" by (simp add: atom.set_map)
+  have "term_atom_vars (term_atom_subst v obj a) = \<Union> ((term_vars o (term_subst v obj)) ` ent a)" by (simp add: atom.set_map)
   moreover 
-  have "\<And>t. v \<notin> (schematic_term_vars (schematic_term_subst v obj t))" 
+  have "\<And>t. v \<notin> (term_vars (term_subst v obj t))" 
     subgoal for t
       by (cases t) auto
     done
   ultimately 
-  show "v \<notin> schematic_term_atom_vars (schematic_term_atom_subst v obj a)" by auto
+  show "v \<notin> term_atom_vars (term_atom_subst v obj a)" by auto
 qed
 
-global_interpretation schematic_formula_syntax: 
-  formula_syntax schematic_term_atom_subst schematic_term_atom_vars schematic_term_atom_objs
-  defines sf_free_vars = schematic_formula_syntax.free_vars
-    and sf_bound_vars = schematic_formula_syntax.bound_vars
-    and sf_objs = schematic_formula_syntax.fobjs
-  by (unfold_locales, auto simp: sa_subst_all)
+lemma term_vars_replaces: "v \<in> term_vars t \<Longrightarrow> c \<in> term_objs (term_subst v c t)"
+  by (cases t) auto
 
-(* These are needed to interpret syntax and semantics of instantiated formulae *)
-fun inst_term_subst::"variable \<Rightarrow> object \<Rightarrow> inst_term \<Rightarrow> inst_term" where
-  "inst_term_subst v obj (inst_term.VAR x) = (if (x = v) then (inst_term.OBJ obj) else inst_term.VAR x)" 
-| "inst_term_subst _ _ (inst_term.OBJ obj) = inst_term.OBJ obj"
-
-abbreviation inst_term_atom_subst where
-"inst_term_atom_subst v obj \<equiv> map_atom (inst_term_subst v obj)"
-
-fun inst_term_vars where
-  "inst_term_vars (inst_term.VAR x) = {x}" 
-| "inst_term_vars (inst_term.OBJ obj) = {}"
-
-definition inst_term_atom_vars::"inst_term atom \<Rightarrow> variable set" where
-"inst_term_atom_vars \<equiv> \<Union> o ent o (map_atom inst_term_vars)"
-
-fun inst_term_objs where
-  "inst_term_objs (inst_term.VAR x) = {}"
-| "inst_term_objs (inst_term.OBJ obj) = {obj}"
-
-definition inst_term_atom_objs where
-"inst_term_atom_objs \<equiv> \<Union> o ent o (map_atom inst_term_objs)"
-
-lemma ia_subst_all: "v \<notin> inst_term_atom_vars (inst_term_atom_subst v obj a)"
+lemma subst_replaces: "v \<in> term_atom_vars a \<Longrightarrow> c \<in> term_atom_objs (term_atom_subst v c a)"
 proof -
-  have "inst_term_atom_vars (inst_term_atom_subst v obj a) = (\<Union> o ent o (map_atom inst_term_vars)) (map_atom (inst_term_subst v obj) a)" unfolding inst_term_atom_vars_def by simp
-  also have "...  = \<Union> (ent (map_atom inst_term_vars (map_atom (inst_term_subst v obj) a)))" by simp
-  also have "... = \<Union> (ent (map_atom (inst_term_vars o (inst_term_subst v obj)) a))" by (simp add: atom.map_comp)
-  finally 
-  have "inst_term_atom_vars (inst_term_atom_subst v obj a) = \<Union> ((inst_term_vars o (inst_term_subst v obj)) ` ent a)" by (simp add: atom.set_map)
-  moreover 
-  have "\<And>t. v \<notin> (inst_term_vars (inst_term_subst v obj t))" 
-    subgoal for t
-      by (cases t) auto
-    done
-  ultimately 
-  show "v \<notin> inst_term_atom_vars (inst_term_atom_subst v obj a)" by auto
+  assume "v \<in> term_atom_vars a"
+  hence "v \<in> \<Union> (term_vars ` ent a)" using tav_alt by blast
+  hence "c \<in> \<Union> ((term_objs o (term_subst v c)) ` ent a)" using term_vars_replaces by auto
+  thus "c \<in> term_atom_objs (term_atom_subst v c a)" using taom_alt tao_alt by blast
 qed
 
 subsection \<open>Closed-World Assumption, Equality, and Negation\<close>
@@ -256,7 +232,7 @@ begin
     "is_predAtom (Atom (predAtm _ _)) = True" | "is_predAtom _ = False"
 
   text \<open>The world model is a set of (atomic) formulas\<close>
-  type_synonym world_model = "inst_formula set"
+  type_synonym world_model = "ground_formula set"
 
   fun subtype_edge where
     "subtype_edge (ty,superty) = (superty,ty)"
@@ -286,22 +262,10 @@ begin
 
 end
 
-sublocale ClosedWorld \<subseteq> formula_semantics 
-    inst_term_atom_subst 
-    inst_term_atom_vars 
-    inst_term_atom_objs
-    t_dom
-  defines
-  semantics (infix "\<Turnstile>" 55) = formula_semantics
-  and
-  entailment (infix "\<TTurnstile>" 55) = formula_entailment
-  and
-  free_vars = free_vars
-  and
-  bound_vars = bound_vars
-  and 
-  objs = fobjs
-  by (unfold_locales, auto simp: ia_subst_all)
+sublocale ClosedWorld \<subseteq> formula_syntax term_atom_subst term_atom_vars term_atom_objs t_dom 
+  defines vars = fvars
+      and objs = fobjs
+  by (unfold_locales, auto simp: subst_subst_all subst_replaces)
 
 context ClosedWorld
 begin
@@ -320,7 +284,7 @@ begin
   definition "wm_basic M \<equiv> \<forall>a\<in>(M::world_model). is_predAtom a"
   
   text \<open>A valuation extracted from the atoms of the world model\<close>
-  definition valuation :: "world_model \<Rightarrow> inst_term atom valuation"
+  definition valuation :: "world_model \<Rightarrow> object atom valuation"
     where "valuation M \<equiv> \<lambda>(predAtm p xs) \<Rightarrow> Atom (predAtm p xs) \<in> M | Eq a b \<Rightarrow> a=b"
 
   value "\<lambda>(predAtm p xs) \<Rightarrow> Atom (predAtm p xs) \<in> M | Eq a b \<Rightarrow> a=b"
@@ -338,7 +302,7 @@ begin
     apply (auto 0 3)[1] (* no blast 0 but instead more general solver 3 in more depth *)
     by (metis atom.exhaust)
 
-  abbreviation cw_entailment::"world_model \<Rightarrow> inst_formula \<Rightarrow> bool" 
+  abbreviation cw_entailment::"world_model \<Rightarrow> ground_formula \<Rightarrow> bool" 
       (infix "\<^sup>c\<TTurnstile>\<^sub>=" 53) where
     "M \<^sup>c\<TTurnstile>\<^sub>= \<phi> \<equiv> close_world M \<TTurnstile> \<phi>"
 
@@ -361,7 +325,7 @@ begin
   find_theorems name: "local*semantics"
 
   lemma valuation_aux_1:
-    fixes M :: world_model and \<phi> :: "inst_formula"
+    fixes M :: world_model and \<phi> :: "ground_formula"
     defines "C \<equiv> close_world M"
     assumes A: "\<forall>\<phi>\<in>C. \<A> \<Turnstile> \<phi>"
     shows "\<A> = valuation M"
@@ -384,13 +348,13 @@ begin
 
   lemma val_imp_close_world: "valuation M \<Turnstile> \<phi> \<Longrightarrow> M \<^sup>c\<TTurnstile>\<^sub>= \<phi>"
     unfolding entailment_def
-    using valuation_aux_1 entailment_def formula_entailment_def
+    using valuation_aux_1 entailment_def
     by auto
 
   lemma close_world_imp_val:
     "wm_basic M \<Longrightarrow> M \<^sup>c\<TTurnstile>\<^sub>= \<phi> \<Longrightarrow> valuation M \<Turnstile> \<phi>"
     unfolding entailment_def
-    using valuation_aux_2 entailment_def formula_entailment_def 
+    using valuation_aux_2 entailment_def 
     by auto
 
   text \<open>Main theorem of this section:
@@ -411,7 +375,7 @@ begin
   
   (* STRIPS formulae don't have quantifiers, negation, or equality.
     (except that true in our language is defined as the negation of false) *)
-  fun is_STRIPS_fmla :: "('tm atom, 'v , 'ty) formula \<Rightarrow> bool" where
+  fun is_STRIPS_fmla :: "('tm atom) formula \<Rightarrow> bool" where
     "is_STRIPS_fmla (Atom (predAtm _ _)) \<longleftrightarrow> True"
   | "is_STRIPS_fmla (\<bottom>) \<longleftrightarrow> True"
   | "is_STRIPS_fmla (\<phi>\<^sub>1 \<^bold>\<and> \<phi>\<^sub>2) \<longleftrightarrow> is_STRIPS_fmla \<phi>\<^sub>1 \<and> is_STRIPS_fmla \<phi>\<^sub>2"
@@ -447,7 +411,7 @@ begin
       using in_close_world_conv valuation_aux_2 apply blast
       using in_close_world_conv valuation_aux_2 by auto
     show ?thesis          
-      using entailment_def formula_entailment_def
+      using entailment_def
       by (auto intro: aux1 aux2)
   qed
   
@@ -476,41 +440,9 @@ subsection \<open>Well-Formedness of PDDL\<close>
 *)
 
 
-
-lemma stav_alt: "schematic_term_atom_vars x = \<Union> (schematic_term_vars ` ent x)" 
-  unfolding schematic_term_atom_vars_def by (simp add: atom.set_map) 
-
-lemma stao_alt: "schematic_term_atom_objs x = \<Union> (schematic_term_objs ` ent x)" 
-  unfolding schematic_term_atom_objs_def by (simp add: atom.set_map) 
-
-lemma itav_alt: "inst_term_atom_vars x = \<Union> (inst_term_vars ` ent x)" 
-  unfolding inst_term_atom_vars_def by (simp add: atom.set_map) 
-
-lemma itao_alt: "inst_term_atom_objs x = \<Union> (inst_term_objs ` ent x)" 
-  unfolding inst_term_atom_objs_def by (simp add: atom.set_map) 
-
-lemma itav_empty: "inst_term_atom_vars x = {} \<longleftrightarrow> (\<forall>e \<in> ent x. inst_term_vars e = {})"
-  using itav_alt by auto
-
-lemma itavm_alt: "inst_term_atom_vars (map_atom f x) = \<Union> ((inst_term_vars o f) ` ent x)"
-  unfolding inst_term_atom_vars_def by (simp add: atom.map_comp atom.set_map)
-
-lemma itaom_alt: "inst_term_atom_objs (map_atom f x) = \<Union> ((inst_term_objs o f) ` ent x)"
-  unfolding inst_term_atom_objs_def by (simp add: atom.map_comp atom.set_map)
-
 fun ty_term::"(variable \<Rightarrow> type option) \<Rightarrow> (object \<Rightarrow> type option) \<Rightarrow> term \<Rightarrow> type option" where
   "ty_term varT objT (term.VAR v) = varT v"
 | "ty_term varT objT (term.CONST c) = objT c"
-
-definition upd_te::"(term \<Rightarrow> type option) \<Rightarrow> variable \<Rightarrow> type \<Rightarrow> term \<Rightarrow> type option" where
-"upd_te te var ty \<equiv> 
-  \<lambda>(term.VAR v) \<Rightarrow> (if (v = var) then Some ty else te (term.VAR v)) |
-  (term.CONST c) \<Rightarrow> te (term.CONST c)"
-
-lemma ty_term_upd: "upd_te (ty_term Q R) v t = ty_term (Q(v\<mapsto>t)) R"
-  unfolding upd_te_def by (auto split: term.split)
-
-find_theorems name: "ty_term"
 
 lemma ty_term_mono: "varT \<subseteq>\<^sub>m varT' \<Longrightarrow> objT \<subseteq>\<^sub>m objT' \<Longrightarrow>
   ty_term varT objT \<subseteq>\<^sub>m ty_term varT' objT'"
@@ -527,25 +459,19 @@ locale ast_domain = ClosedWorld "type_env D"
   defines "t \<equiv> type_env D"
 begin
 
-(* having to re-declare syntax is weird *)
-notation entailment (infix "\<TTurnstile>" 55)
-notation semantics (infix "\<Turnstile>" 55)
-notation cw_entailment (infix "\<^sup>c\<TTurnstile>\<^sub>=" 55)
-
-
   text \<open>The signature is a partial function that maps the predicates
     of the domain to lists of argument types.\<close>
   definition sig :: "predicate \<rightharpoonup> type list" where
     "sig \<equiv> map_of (map (\<lambda>PredDecl p n \<Rightarrow> (p,n)) (predicates D))"
 
-type_synonym ('ent) ty_ent = "'ent \<rightharpoonup> type"
+  type_synonym ('ent) ty_ent = "'ent \<rightharpoonup> type"
 
   text \<open>For the next few definitions, we fix a partial function that maps
     a polymorphic entity type @{typ "'e"} to types. An entity can be
     instantiated by variables or objects later.\<close>
   context
-    fixes ty_ent :: "'ent ty_ent"  \<comment> \<open>Entity's type, None if invalid\<close>
-begin
+    fixes ty_ent :: "'ent \<rightharpoonup> type"  \<comment> \<open>Entity's type, None if invalid\<close>
+  begin
 
     text \<open>Checks whether an entity has a given type\<close>
     definition is_of_type :: "'ent \<Rightarrow> type \<Rightarrow> bool" where
@@ -569,55 +495,40 @@ begin
     fun wf_atom :: "'ent atom \<Rightarrow> bool" where
       "wf_atom (predAtm p vs) \<longleftrightarrow> wf_pred_atom (p,vs)"
     | "wf_atom (Eq a b) \<longleftrightarrow> ty_ent a \<noteq> None \<and> ty_ent b \<noteq> None"
-  end \<comment> \<open>Context fixing \<open>ty_ent\<close>\<close>
 
-  context
-    fixes upd :: "'ent ty_ent \<Rightarrow> 'var \<Rightarrow> 'type \<Rightarrow> 'ent ty_ent"
-  begin
     text \<open>A formula is well-formed if it consists of valid atoms,
       and does not contain negations, except for the encoding \<open>\<^bold>\<not>\<bottom>\<close> of true.
-      Ignore this
     \<close>
+    fun wf_fmla :: "('ent atom) formula \<Rightarrow> bool" where
+      "wf_fmla (Atom a) \<longleftrightarrow> wf_atom a"
+    | "wf_fmla (\<bottom>) \<longleftrightarrow> True"
+    | "wf_fmla (\<phi>1 \<^bold>\<and> \<phi>2) \<longleftrightarrow> (wf_fmla \<phi>1 \<and> wf_fmla \<phi>2)"
+    | "wf_fmla (\<phi>1 \<^bold>\<or> \<phi>2) \<longleftrightarrow> (wf_fmla \<phi>1 \<and> wf_fmla \<phi>2)"
+    | "wf_fmla (\<^bold>\<not>\<phi>) \<longleftrightarrow> wf_fmla \<phi>"
+    | "wf_fmla (\<phi>1 \<^bold>\<rightarrow> \<phi>2) \<longleftrightarrow> (wf_fmla \<phi>1 \<and> wf_fmla \<phi>2)"
 
-    fun wf_fmla :: "'ent ty_ent \<Rightarrow> ('ent atom, 'var, 'type) formula \<Rightarrow> bool" where
-      "wf_fmla te (Atom a) \<longleftrightarrow> wf_atom te a"
-    | "wf_fmla te (\<bottom>) \<longleftrightarrow> True"
-    | "wf_fmla te (\<phi>1 \<^bold>\<and> \<phi>2) \<longleftrightarrow> (wf_fmla te \<phi>1 \<and> wf_fmla te \<phi>2)"
-    | "wf_fmla te (\<phi>1 \<^bold>\<or> \<phi>2) \<longleftrightarrow> (wf_fmla te \<phi>1 \<and> wf_fmla te \<phi>2)"
-    | "wf_fmla te (\<^bold>\<not>\<phi>) \<longleftrightarrow> wf_fmla te \<phi>"
-    | "wf_fmla te (\<phi>1 \<^bold>\<rightarrow> \<phi>2) \<longleftrightarrow> (wf_fmla te \<phi>1 \<and> wf_fmla te \<phi>2)"
-    | "wf_fmla te (\<^bold>\<forall>\<^sub>\<tau> v. \<phi>) \<longleftrightarrow> (wf_fmla (upd te v \<tau>) \<phi>)"
-    | "wf_fmla te (\<^bold>\<exists>\<^sub>\<tau> v. \<phi>) \<longleftrightarrow> (wf_fmla (upd te v \<tau>) \<phi>)" 
-
-    (* When considering the well-typedness of formulae, when variables 
-       are bound, we update the type. *)
-
-    (* this no longer holds *)
-    (* lemma "wf_fmla \<phi> = (\<forall>a\<in>formula.atoms \<phi>. wf_atom a)"
-      by (induction \<phi>) auto *)
+    lemma "wf_fmla \<phi> = (\<forall>a\<in>atoms \<phi>. wf_atom a)"
+      by (induction \<phi>) auto
 
     (*lemma wf_fmla_add_simps[simp]: "wf_fmla (\<^bold>\<not>\<phi>) \<longleftrightarrow> \<phi>=\<bottom>"
       by (cases \<phi>) auto*)
 
-
     text \<open>Special case for a well-formed atomic predicate formula\<close>
     fun wf_fmla_atom where
-      "wf_fmla_atom te (Atom (predAtm a vs)) \<longleftrightarrow> wf_pred_atom te (a,vs)"
-    | "wf_fmla_atom _ _ \<longleftrightarrow> False"
+      "wf_fmla_atom (Atom (predAtm a vs)) \<longleftrightarrow> wf_pred_atom (a,vs)"
+    | "wf_fmla_atom _ \<longleftrightarrow> False"
 
-    (* same as the above *)
-    lemma wf_fmla_atom_alt: "wf_fmla_atom te \<phi> \<longleftrightarrow> is_predAtom \<phi> \<and> wf_fmla te \<phi>"
-      by (cases "(te, \<phi>)" rule: wf_fmla_atom.cases) auto
+    lemma wf_fmla_atom_alt: "wf_fmla_atom \<phi> \<longleftrightarrow> is_predAtom \<phi> \<and> wf_fmla \<phi>"
+      by (cases \<phi> rule: wf_fmla_atom.cases) auto
 
-    thm wf_fmla_atom.cases
     text \<open>An effect is well-formed if the added and removed formulas
       are atomic\<close>
     fun wf_effect where
-      "wf_effect te (Effect a d) \<longleftrightarrow>
-          (\<forall>ae\<in>set a. wf_fmla_atom te ae)
-        \<and> (\<forall>de\<in>set d. wf_fmla_atom te de)"
+      "wf_effect (Effect a d) \<longleftrightarrow>
+          (\<forall>ae\<in>set a. wf_fmla_atom ae)
+        \<and> (\<forall>de\<in>set d. wf_fmla_atom de)"
 
-  end \<comment> \<open>context fixing the update function for ty_ent\<close>
+  end \<comment> \<open>Context fixing \<open>ty_ent\<close>\<close>
 
   definition constT :: "object \<rightharpoonup> type" where
     "constT \<equiv> map_of (consts t)"
@@ -631,7 +542,7 @@ begin
         tyt = ty_term (map_of params) constT
       in
         distinct (map fst params)
-      \<and> wf_fmla upd_te tyt pre
+      \<and> wf_fmla tyt pre
       \<and> wf_effect tyt eff)"
              
   text \<open>A type is well-formed if it consists only of declared primitive types,
@@ -657,8 +568,8 @@ begin
       wf_types
     \<and> distinct (map (predicate_decl.pred) (predicates D))
     \<and> (\<forall>p\<in>set (predicates D). wf_predicate_decl p)
-    \<and> distinct (map fst (consts t))
-    \<and> (\<forall>(n,T)\<in>set (consts t). wf_type T)
+    \<and> distinct (map fst (consts (type_env D)))
+    \<and> (\<forall>(n,T)\<in>set (consts (type_env D)). wf_type T)
     \<and> distinct (map ast_action_schema.name (actions D))
     \<and> (\<forall>a\<in>set (actions D). wf_action_schema a)
     "
@@ -676,14 +587,14 @@ begin
   text \<open>It seems to be agreed upon that, in case of a contradictory effect,
     addition overrides deletion. We model this behaviour by first executing
     the deletions, and then the additions.\<close>
-  fun apply_effect :: "inst_effect \<Rightarrow> world_model \<Rightarrow> world_model"
+  fun apply_effect :: "ground_effect \<Rightarrow> world_model \<Rightarrow> world_model"
   where
      "apply_effect (Effect a d) s = (s - set d) \<union> (set a)"
 
   text \<open>Execute a ground action\<close>
-  definition execute_inst_action :: "inst_action \<Rightarrow> world_model \<Rightarrow> world_model"
+  definition execute_ground_action :: "ground_action \<Rightarrow> world_model \<Rightarrow> world_model"
   where
-    "execute_inst_action a M = apply_effect (effect a) M"
+    "execute_ground_action a M = apply_effect (effect a) M"
 
 
   text \<open>Predicate to model that the given list of action instances is
@@ -695,49 +606,24 @@ begin
      models, as done in [Lif87].
   \<close>
 
-  fun inst_action_path
-    :: "world_model \<Rightarrow> inst_action list \<Rightarrow> world_model \<Rightarrow> bool"
+  fun ground_action_path
+    :: "world_model \<Rightarrow> ground_action list \<Rightarrow> world_model \<Rightarrow> bool"
   where
-    "inst_action_path M [] M' = (M = M')"
-  | "inst_action_path M (\<alpha>#\<alpha>s) M' = (M \<^sup>c\<TTurnstile>\<^sub>= precondition \<alpha>
-    \<and> inst_action_path (execute_inst_action \<alpha> M) \<alpha>s M')"
+    "ground_action_path M [] M' = (M = M')"
+  | "ground_action_path M (\<alpha>#\<alpha>s) M' = (M \<^sup>c\<TTurnstile>\<^sub>= precondition \<alpha>
+    \<and> ground_action_path (execute_ground_action \<alpha> M) \<alpha>s M')"
 
   text \<open>Function equations as presented in paper,
-    with inlined @{const execute_inst_action}.\<close>
-  lemma inst_action_path_in_paper:
-    "inst_action_path M [] M' \<longleftrightarrow> (M = M')"
-    "inst_action_path M (\<alpha>#\<alpha>s) M' \<longleftrightarrow> M \<^sup>c\<TTurnstile>\<^sub>= precondition \<alpha>
-    \<and> (inst_action_path (apply_effect (effect \<alpha>) M) \<alpha>s M')"
-    by (auto simp: execute_inst_action_def)
+    with inlined @{const execute_ground_action}.\<close>
+  lemma ground_action_path_in_paper:
+    "ground_action_path M [] M' \<longleftrightarrow> (M = M')"
+    "ground_action_path M (\<alpha>#\<alpha>s) M' \<longleftrightarrow> M \<^sup>c\<TTurnstile>\<^sub>= precondition \<alpha>
+    \<and> (ground_action_path (apply_effect (effect \<alpha>) M) \<alpha>s M')"
+    by (auto simp: execute_ground_action_def)
 
-  thm inst_action_path_in_paper
+  thm ground_action_path_in_paper
 
 end \<comment> \<open>Context of \<open>ast_domain\<close>\<close>
-
-
-fun ty_inst_term::"(variable \<Rightarrow> type option) \<Rightarrow> (object \<Rightarrow> type option) \<Rightarrow> inst_term \<Rightarrow> type option" where
-  "ty_inst_term varT objT (inst_term.VAR v) = varT v"
-| "ty_inst_term varT objT (inst_term.OBJ obj) = objT obj"
-
-definition upd_inst_te::"(inst_term \<Rightarrow> type option) \<Rightarrow> variable \<Rightarrow> type \<Rightarrow> inst_term \<Rightarrow> type option" where
-"upd_inst_te te var ty \<equiv> 
-  \<lambda>(inst_term.VAR v) \<Rightarrow> (if (v = var) then Some ty else te (inst_term.VAR v)) |
-  (inst_term.OBJ c) \<Rightarrow> te (inst_term.OBJ c)"
-
-lemma ty_inst_term_upd: "upd_inst_te (ty_inst_term Q R) v t = ty_inst_term (Q(v \<mapsto> t)) R"
-  unfolding upd_inst_te_def
-  by (auto split: inst_term.splits)
-
-find_theorems name: "ty_term"
-
-lemma ty_inst_term_mono: "varT \<subseteq>\<^sub>m varT' \<Longrightarrow> objT \<subseteq>\<^sub>m objT' \<Longrightarrow>
-  ty_inst_term varT objT \<subseteq>\<^sub>m ty_inst_term varT' objT'"
-  apply (rule map_leI)
-  subgoal for x v
-    apply (cases x)
-    apply (auto dest: map_leD)
-    done
-  done
 
 text \<open>We fix a problem, and also include the definitions for the domain
   of this problem.\<close>
@@ -758,18 +644,18 @@ begin
     done
 
   definition wf_fact :: "fact \<Rightarrow> bool" where
-    "wf_fact = wf_pred_atom (ty_inst_term (\<lambda>_. None) objT)"
-  (* TODO: what is a fact? My assumption is that they are not quantified. *)
-
+    "wf_fact = wf_pred_atom objT"
   text \<open>This definition is needed for well-formedness of the initial model,
     and forward-references to the concept of world model.
   \<close>
   (* What makes a world-model well-formed? Since the initial state is essentially
       equivalent to the effect of a non-action, it being well-formed means, that it
       is unquantified. *)
-definition wf_world_model::
-"inst_formula set \<Rightarrow> bool" where
-    "wf_world_model M = (\<forall>f\<in>M. wf_fmla_atom (ty_inst_term (\<lambda>_. None) objT) f)"
+  definition wf_world_model::"ground_formula set \<Rightarrow> bool" where
+    "wf_world_model M = (\<forall>f\<in>M. wf_fmla_atom objT f)"
+
+  definition wf_goal::"schematic_formula \<Rightarrow> bool" where
+    "wf_goal = wf_fmla (ty_term (Map.empty) constT)"
 
   (*Note: current semantics assigns each object a unique type *)
   definition wf_problem where
@@ -779,22 +665,18 @@ definition wf_world_model::
     \<and> (\<forall>(n,T)\<in>set (objects P). wf_type T)
     \<and> distinct (init P)
     \<and> wf_world_model (set (init P))
-    \<and> wf_fmla upd_inst_te (ty_inst_term (\<lambda>_.None) objT) (goal P)
+    \<and> wf_goal (goal P)
     "
 
-  definition wf_inst_fmla::"inst_formula \<Rightarrow> bool" where
-  "wf_inst_fmla f \<equiv> wf_fmla upd_inst_te (ty_inst_term (\<lambda>_. None) objT) f"
-
-  fun wf_inst_fmla_atom::"inst_formula \<Rightarrow> bool" where
-    "wf_inst_fmla_atom (Atom (predAtm a vs)) = wf_inst_fmla (Atom (predAtm a vs))"
-  | "wf_inst_fmla_atom _ = False"
-
-  fun wf_effect_inst :: "inst_effect \<Rightarrow> bool" where
+  fun wf_effect_inst :: "object ast_effect \<Rightarrow> bool" where
     "wf_effect_inst (Effect (a) (d))
-      \<longleftrightarrow> (\<forall>a\<in>set a \<union> set d. wf_inst_fmla_atom a)"
+      \<longleftrightarrow> (\<forall>a\<in>set a \<union> set d. wf_fmla_atom objT a)"
+
+  lemma wf_effect_inst_alt: "wf_effect_inst eff = wf_effect objT eff"
+    by (cases eff) auto
 
   text \<open>The following section reasons shows that well-formed instantiated formulae do not have free
-        variables and relates wf_inst_fmla to wf_inst_fmla_atom. It also contains a few lemmas proving
+        variables and relates wf_ground_fmla to wf_ground_fmla_atom. It also contains a few lemmas proving
         similar results for schematic formulas and terms\<close>
 
   lemma wf_imp_ent_typed:
@@ -821,41 +703,6 @@ definition wf_world_model::
   next
     case (Eq x y)
     thus ?thesis using wf by auto
-  qed
-
-  text \<open>The following two lemmas concern the variables present in a schematic atom
-        and an instantiated atom\<close>
-
-  lemma wf_schematic_atom_vars: "wf_atom (ty_term Q constT) a \<Longrightarrow> schematic_term_atom_vars a \<subseteq> dom Q"
-  proof (rule subsetI)
-    fix v
-    assume wf: "wf_atom (ty_term Q constT) a"
-    assume "v \<in> schematic_term_atom_vars a"
-    then obtain e where
-      e: "e \<in> ent a" 
-      "v \<in> schematic_term_vars e" 
-      by (auto simp: stav_alt)
-    hence "e = term.VAR v" by (cases e rule: term.exhaust) auto
-    moreover
-    have "ty_term Q constT e \<noteq> None" using e wf_imp_ent_typed wf by fastforce
-    ultimately
-    show "v \<in> dom Q" by auto
-  qed
-  
-  lemma wf_inst_atom_vars: "wf_atom (ty_inst_term Q objT) a \<Longrightarrow> inst_term_atom_vars a \<subseteq> dom Q"
-  proof (rule subsetI)
-    fix v
-    assume wf: "wf_atom (ty_inst_term Q objT) a"
-    assume "v \<in> inst_term_atom_vars a"
-    then obtain e where
-      e: "e \<in> ent a" 
-      "v \<in> inst_term_vars e" 
-      by (auto simp: itav_alt)
-    hence "e = inst_term.VAR v" by (cases e rule: inst_term.exhaust) auto
-    moreover
-    have "ty_inst_term Q objT e \<noteq> None" using e wf_imp_ent_typed wf by fastforce
-    ultimately
-    show "v \<in> dom Q" by auto
   qed
 
   text \<open>This section proves that under certain circumstances, namely the type environments assigning
@@ -897,14 +744,18 @@ definition wf_world_model::
     case [simp]: (Eq x y)
     then show ?thesis using assms by auto
   qed
-  
+
+  lemma list_all2_ty':
+  fixes xs Ts
+    assumes "\<forall>x \<in> set xs. Q x = R x" 
+    shows "list_all2 (is_of_type Q) xs Ts =  list_all2 (is_of_type R) xs Ts"
+  using list_all2_ty assms by metis
   
   lemma map_le_imp_same_type: 
     assumes le: "Q \<subseteq>\<^sub>m R" 
         and wf: "wf_atom Q a"
     shows "\<forall>e \<in> ent a. Q e = R e"
     using wf_imp_ent_typed[OF wf] map_leD le by fastforce
-
 
   lemma wf_atom_mono:
     assumes SS: "tys \<subseteq>\<^sub>m tys'"
@@ -922,206 +773,131 @@ definition wf_world_model::
       [simp]: "a = Atom (predAtm p vs)"
       "wf_atom tys (predAtm p vs)"
       using WF
-      by (cases "(tys, a)" rule: wf_fmla_atom.cases) auto
+      by (cases "a" rule: wf_fmla_atom.cases) auto
     from wf_atom_mono[OF SS this(2)]
     show ?thesis by simp
   qed
-  
-  lemma wf_inst_atom_mono: 
-    assumes le: "Q \<subseteq>\<^sub>m R" 
-        and wf: "wf_atom (ty_inst_term Q objT) a"
-      shows "wf_atom (ty_inst_term R objT) a"
-    using ty_inst_term_mono[OF le map_le_refl[of objT], THEN wf_atom_mono] wf
-    by blast
 
-  lemma inst_term_vars_restr_same_type: "\<forall>e \<in> ent a. (ty_inst_term Q objT) e = (ty_inst_term (Q |` (inst_term_atom_vars a)) objT) e"
+ lemma term_vars_restr_same_type: "\<forall>e \<in> ent a. (ty_term Q cT) e = (ty_term (Q |` (term_atom_vars a)) cT) e"
   proof
     fix e
     assume "e \<in> ent a"
-    hence "inst_term_vars e \<subseteq> inst_term_atom_vars a" using itav_alt by blast
-    hence "(ty_inst_term (Q |` (inst_term_vars e)) objT) e = (ty_inst_term (Q |` (inst_term_atom_vars a)) objT) e" by (cases e) auto
+    hence "term_vars e \<subseteq> term_atom_vars a" using tav_alt by blast
+    hence "(ty_term (Q |` (term_vars e)) cT) e = (ty_term (Q |` (term_atom_vars a)) cT) e" by (cases e) auto
     moreover
-    have "(ty_inst_term Q objT) e = (ty_inst_term (Q |` (inst_term_vars e)) objT) e" by (cases e) auto
+    have "(ty_term Q cT) e = (ty_term (Q |` (term_vars e)) cT) e" by (cases e) auto
     ultimately 
-    show "(ty_inst_term Q objT) e = (ty_inst_term (Q |` (inst_term_atom_vars a)) objT) e" by argo
+    show "(ty_term Q cT) e = (ty_term (Q |` (term_atom_vars a)) cT) e" by argo
   qed
 
   lemma wf_atom_restr: 
-    assumes wf: "wf_atom (ty_inst_term Q objT) a" 
-      shows "wf_atom (ty_inst_term (Q |` (inst_term_atom_vars a)) objT) a"
-    using same_type_imp_wf_eq[OF inst_term_vars_restr_same_type wf]
+    assumes wf: "wf_atom (ty_term Q cT) a" 
+      shows "wf_atom (ty_term (Q |` (term_atom_vars a)) cT) a"
+    using same_type_imp_wf_eq[OF term_vars_restr_same_type wf]
     .
 
+  lemma wf_schematic_atom_vars: "wf_atom (ty_term Q cT) a \<Longrightarrow> term_atom_vars a \<subseteq> dom Q"
+  proof (rule subsetI)
+    fix v
+    assume wf: "wf_atom (ty_term Q cT) a"
+    assume "v \<in> term_atom_vars a"
+    then obtain e where
+      e: "e \<in> ent a" 
+      "v \<in> term_vars e" 
+      by (auto simp: tav_alt)
+    hence "e = term.VAR v" by (cases e rule: term.exhaust) auto
+    moreover
+    have "ty_term Q cT e \<noteq> None" using e wf_imp_ent_typed wf by fastforce
+    ultimately
+    show "v \<in> dom Q" by auto
+  qed
+
   text \<open>The type environment must contain a type for all free variables in a formula.\<close>
-  lemma wf_schematic_fmla_free_vars: "wf_fmla upd_te (ty_term Q constT) \<phi> \<Longrightarrow> sf_free_vars \<phi> \<subseteq> dom Q"
-  proof (induction \<phi> arbitrary: Q)
-    case (Atom x)
-    then show ?case using wf_schematic_atom_vars by simp
-  next
-    case (Exists t x \<phi>)
-    hence "wf_fmla upd_te (ty_term (Q(x \<mapsto> t)) constT) \<phi>" using ty_term_upd by simp
-    hence "sf_free_vars \<phi> \<subseteq> dom (Q(x \<mapsto> t))" using Exists.IH by blast
-    then show ?case by auto
-  next
-    case (All t x \<phi>)
-    hence "wf_fmla upd_te (ty_term (Q(x \<mapsto> t)) constT) \<phi>" using ty_term_upd by simp
-    hence "sf_free_vars \<phi> \<subseteq> dom (Q(x \<mapsto> t))" using All.IH by blast                
-    then show ?case by auto
-  qed simp_all
+  lemma wf_fmla_vars: "wf_fmla (ty_term Q cT) \<phi> \<Longrightarrow> vars \<phi> \<subseteq> dom Q"
+    using wf_schematic_atom_vars
+    by (induction \<phi>) auto
+
+  find_theorems "?a \<subseteq>\<^sub>m ?a"
+
+  lemma wf_fmla_fw: 
+    assumes "wf_fmla (ty_term Q cT) \<phi>"
+            "Q \<subseteq>\<^sub>m R"
+    shows "wf_fmla (ty_term R cT) \<phi>"
+    using wf_atom_mono[OF ty_term_mono[OF assms(2) map_le_refl[of cT]]] assms(1)
+    apply (induction \<phi>) by auto
   
-  lemma wf_inst_fmla_free_vars: "wf_fmla upd_inst_te (ty_inst_term Q objT) \<phi> \<Longrightarrow> free_vars \<phi> \<subseteq> dom Q"
-  proof (induction \<phi> arbitrary: Q)
-    case (Atom x)
-    then show ?case using wf_inst_atom_vars by simp
-  next
-    case (Exists t x \<phi>)
-    hence "wf_fmla upd_inst_te (ty_inst_term (Q(x \<mapsto> t)) objT) \<phi>" using ty_inst_term_upd by simp
-    hence "free_vars \<phi> \<subseteq> dom (Q(x \<mapsto> t))" using Exists.IH by blast
-    then show ?case by auto
-  next
-    case (All t x \<phi>)
-    hence "wf_fmla upd_inst_te (ty_inst_term (Q(x \<mapsto> t)) objT) \<phi>" using ty_inst_term_upd by simp
-    hence "free_vars \<phi> \<subseteq> dom (Q(x \<mapsto> t))" using All.IH by blast                  
-    then show ?case by auto
-  qed simp_all
-  
-  lemma wf_fmla_fw: "Q \<subseteq>\<^sub>m R \<Longrightarrow> wf_fmla upd_inst_te (ty_inst_term Q objT) \<phi> 
-    \<Longrightarrow> wf_fmla upd_inst_te (ty_inst_term R objT) \<phi>"
-  proof (induction \<phi> arbitrary: Q R)
-    case (Atom x)
-    then show ?case using wf_inst_atom_mono by simp
-  next
-    case (Exists t x \<phi>)
-    then show ?case 
-      using Exists.IH[OF map_le_upd[OF \<open>Q \<subseteq>\<^sub>m R\<close>, of x "Some t"]] ty_inst_term_upd
-      by fastforce
-  next
-    case (All t x \<phi>)
-    then show ?case 
-      using All.IH[OF map_le_upd[OF \<open>Q \<subseteq>\<^sub>m R\<close>, of x "Some t"]] ty_inst_term_upd
-      by fastforce
-  qed auto
-  
-  lemma wf_fmla_restr': "wf_fmla upd_inst_te (ty_inst_term Q objT) \<phi> 
-    \<Longrightarrow> wf_fmla upd_inst_te (ty_inst_term (Q |` (free_vars \<phi>)) objT) \<phi>"
+  lemma wf_fmla_restr': "wf_fmla (ty_term Q cT) \<phi> 
+    \<Longrightarrow> wf_fmla (ty_term (Q |` (vars \<phi>)) cT) \<phi>"
   proof (induction \<phi> arbitrary: Q)
     case (Atom x)
     then show ?case using wf_atom_restr by simp
   next
-    case Bot
-    then show ?case by simp
-  next
-    case (Not \<phi>)
-    then show ?case by simp
-  next
     case (And \<phi>1 \<phi>2)
-    have "free_vars \<phi>1 \<subseteq> free_vars (\<phi>1 \<^bold>\<and> \<phi>2)" by simp
-    hence "Q |` free_vars \<phi>1 \<subseteq>\<^sub>m Q |` free_vars (\<phi>1 \<^bold>\<and> \<phi>2)"
-      using map_restrict_mono[of "free_vars \<phi>1" _ Q] by blast
-    hence "wf_fmla upd_inst_te (ty_inst_term (Q |` free_vars (\<phi>1 \<^bold>\<and> \<phi>2)) objT) \<phi>1"
+    have "vars \<phi>1 \<subseteq> vars (\<phi>1 \<^bold>\<and> \<phi>2)" by simp
+    hence "Q |` vars \<phi>1 \<subseteq>\<^sub>m Q |` vars (\<phi>1 \<^bold>\<and> \<phi>2)"
+      using map_restrict_mono[of "vars \<phi>1" _ Q] by blast
+    hence "wf_fmla (ty_term (Q |` vars (\<phi>1 \<^bold>\<and> \<phi>2)) cT) \<phi>1"
       using wf_fmla_fw And by fastforce
     moreover
-    have "free_vars \<phi>2 \<subseteq> free_vars (\<phi>1 \<^bold>\<and> \<phi>2)" by simp
-    hence "Q |` free_vars \<phi>2 \<subseteq>\<^sub>m Q |` free_vars (\<phi>1 \<^bold>\<and> \<phi>2)"
+    have "vars \<phi>2 \<subseteq> vars (\<phi>1 \<^bold>\<and> \<phi>2)" by simp
+    hence "Q |` vars \<phi>2 \<subseteq>\<^sub>m Q |` vars (\<phi>1 \<^bold>\<and> \<phi>2)"
       using map_restrict_mono by blast
-    hence "wf_fmla upd_inst_te (ty_inst_term (Q |` free_vars (\<phi>1 \<^bold>\<and> \<phi>2)) objT) \<phi>2"
+    hence "wf_fmla (ty_term (Q |` vars (\<phi>1 \<^bold>\<and> \<phi>2)) cT) \<phi>2"
       using wf_fmla_fw And by fastforce
     ultimately
     show ?case by simp
   next
     case (Or \<phi>1 \<phi>2)
-    have "free_vars \<phi>1 \<subseteq> free_vars (\<phi>1 \<^bold>\<or> \<phi>2)" by simp
-    hence "Q |` free_vars \<phi>1 \<subseteq>\<^sub>m Q |` free_vars (\<phi>1 \<^bold>\<or> \<phi>2)"
-      using map_restrict_mono[of "free_vars \<phi>1" _ Q] by blast
-    hence "wf_fmla upd_inst_te (ty_inst_term (Q |` free_vars (\<phi>1 \<^bold>\<or> \<phi>2)) objT) \<phi>1"
+    have "vars \<phi>1 \<subseteq> vars (\<phi>1 \<^bold>\<or> \<phi>2)" by simp
+    hence "Q |` vars \<phi>1 \<subseteq>\<^sub>m Q |` vars (\<phi>1 \<^bold>\<or> \<phi>2)"
+      using map_restrict_mono[of "vars \<phi>1" _ Q] by blast
+    hence "wf_fmla (ty_term (Q |` vars (\<phi>1 \<^bold>\<or> \<phi>2)) cT) \<phi>1"
       using wf_fmla_fw Or by fastforce
     moreover
-    have "free_vars \<phi>2 \<subseteq> free_vars (\<phi>1 \<^bold>\<or> \<phi>2)" by simp
-    hence "Q |` free_vars \<phi>2 \<subseteq>\<^sub>m Q |` free_vars (\<phi>1 \<^bold>\<or> \<phi>2)"
+    have "vars \<phi>2 \<subseteq> vars (\<phi>1 \<^bold>\<or> \<phi>2)" by simp
+    hence "Q |` vars \<phi>2 \<subseteq>\<^sub>m Q |` vars (\<phi>1 \<^bold>\<or> \<phi>2)"
       using map_restrict_mono by blast
-    hence "wf_fmla upd_inst_te (ty_inst_term (Q |` free_vars (\<phi>1 \<^bold>\<or> \<phi>2)) objT) \<phi>2"
+    hence "wf_fmla (ty_term (Q |` vars (\<phi>1 \<^bold>\<or> \<phi>2)) cT) \<phi>2"
       using wf_fmla_fw Or by fastforce
     ultimately
     show ?case by simp
   next
     case (Imp \<phi>1 \<phi>2)
-    have "free_vars \<phi>1 \<subseteq> free_vars (\<phi>1 \<^bold>\<rightarrow> \<phi>2)" by simp
-    hence "Q |` free_vars \<phi>1 \<subseteq>\<^sub>m Q |` free_vars (\<phi>1 \<^bold>\<rightarrow> \<phi>2)"
-      using map_restrict_mono[of "free_vars \<phi>1" _ Q] by blast
-    hence "wf_fmla upd_inst_te (ty_inst_term (Q |` free_vars (\<phi>1 \<^bold>\<rightarrow> \<phi>2)) objT) \<phi>1"
+    have "vars \<phi>1 \<subseteq> vars (\<phi>1 \<^bold>\<rightarrow> \<phi>2)" by simp
+    hence "Q |` vars \<phi>1 \<subseteq>\<^sub>m Q |` vars (\<phi>1 \<^bold>\<rightarrow> \<phi>2)"
+      using map_restrict_mono[of "vars \<phi>1" _ Q] by blast
+    hence "wf_fmla (ty_term (Q |` vars (\<phi>1 \<^bold>\<rightarrow> \<phi>2)) cT) \<phi>1"
       using wf_fmla_fw Imp by fastforce
     moreover
-    have "free_vars \<phi>2 \<subseteq> free_vars (\<phi>1 \<^bold>\<rightarrow> \<phi>2)" by simp
-    hence "Q |` free_vars \<phi>2 \<subseteq>\<^sub>m Q |` free_vars (\<phi>1 \<^bold>\<rightarrow> \<phi>2)"
+    have "vars \<phi>2 \<subseteq> vars (\<phi>1 \<^bold>\<rightarrow> \<phi>2)" by simp
+    hence "Q |` vars \<phi>2 \<subseteq>\<^sub>m Q |` vars (\<phi>1 \<^bold>\<rightarrow> \<phi>2)"
       using map_restrict_mono by blast
-    hence "wf_fmla upd_inst_te (ty_inst_term (Q |` free_vars (\<phi>1 \<^bold>\<rightarrow> \<phi>2)) objT) \<phi>2"
+    hence "wf_fmla (ty_term (Q |` vars (\<phi>1 \<^bold>\<rightarrow> \<phi>2)) cT) \<phi>2"
       using wf_fmla_fw Imp by fastforce
     ultimately
     show ?case by simp
-  next
-    case (Exists t x \<phi>)
-    hence "wf_fmla upd_inst_te (ty_inst_term (Q(x \<mapsto> t)) objT) \<phi>" using ty_inst_term_upd by simp
-    hence 1: "wf_fmla upd_inst_te (ty_inst_term (Q(x \<mapsto> t) |` (free_vars \<phi>)) objT) \<phi>" using Exists.IH by blast
-    have "Q (x \<mapsto> t) |` (free_vars \<phi>) \<subseteq>\<^sub>m (Q |` (free_vars (\<^bold>\<exists>\<^sub>t x. \<phi>))) (x \<mapsto> t)"
-      unfolding restrict_map_def map_le_def by (cases "x \<in> free_vars \<phi>") auto
-    from wf_fmla_fw[OF this] 1
-    have "wf_fmla upd_inst_te (ty_inst_term ((Q |` free_vars (\<^bold>\<exists>\<^sub>t x. \<phi>))(x \<mapsto> t)) objT) \<phi>" .
-    thus ?case using ty_inst_term_upd by simp
-  next
-    case (All t x \<phi>)
-    hence "wf_fmla upd_inst_te (ty_inst_term (Q(x \<mapsto> t)) objT) \<phi>" using ty_inst_term_upd by simp
-    hence 1: "wf_fmla upd_inst_te (ty_inst_term (Q(x \<mapsto> t) |` (free_vars \<phi>)) objT) \<phi>" using All.IH by blast
-    have "Q (x \<mapsto> t) |` (free_vars \<phi>) \<subseteq>\<^sub>m (Q |` (free_vars (\<^bold>\<forall>\<^sub>t x. \<phi>))) (x \<mapsto> t)"
-      unfolding restrict_map_def map_le_def by (cases "x \<in> free_vars \<phi>") auto
-    from wf_fmla_fw[OF this] 1
-    have "wf_fmla upd_inst_te (ty_inst_term ((Q |` free_vars (\<^bold>\<forall>\<^sub>t x. \<phi>))(x \<mapsto> t)) objT) \<phi>" .
-    thus ?case using ty_inst_term_upd by simp
-  qed 
-  
-  lemma wf_fmla_restr: "wf_fmla upd_inst_te (ty_inst_term Q objT) \<phi> 
-    \<longleftrightarrow> wf_fmla upd_inst_te (ty_inst_term (Q |` (free_vars \<phi>)) objT) \<phi>"
+  qed auto
+   
+  lemma wf_fmla_restr: "wf_fmla (ty_term Q cT) \<phi> 
+    \<longleftrightarrow> wf_fmla (ty_term (Q |` (vars \<phi>)) cT) \<phi>"
     using wf_fmla_restr' wf_fmla_fw map_restrict_less
     by blast
   
-  lemma wf_fmla_bw: "Q \<subseteq>\<^sub>m R \<Longrightarrow> free_vars \<phi> \<subseteq> dom Q
-    \<Longrightarrow> wf_fmla upd_inst_te (ty_inst_term R objT) \<phi> 
-    \<longleftrightarrow> wf_fmla upd_inst_te (ty_inst_term Q objT) \<phi>"
+  lemma wf_fmla_bw: "Q \<subseteq>\<^sub>m R \<Longrightarrow> vars \<phi> \<subseteq> dom Q
+    \<Longrightarrow> wf_fmla (ty_term R cT) \<phi> 
+    \<longleftrightarrow> wf_fmla (ty_term Q cT) \<phi>"
     using wf_fmla_restr[of R] sym[OF wf_fmla_restr[of Q]] map_le_restr
     by metis
   
-  lemma wf_inst_fmla_alt_lemma: "Q \<subseteq>\<^sub>m R \<Longrightarrow> wf_fmla upd_inst_te (ty_inst_term Q objT) \<phi> 
-    \<longleftrightarrow> wf_fmla upd_inst_te (ty_inst_term R objT) \<phi> \<and> free_vars \<phi> \<subseteq> dom Q"
-    using wf_fmla_fw wf_inst_fmla_free_vars wf_fmla_bw 
+  lemma wf_fmla_alt_lemma: "Q \<subseteq>\<^sub>m R \<Longrightarrow> wf_fmla (ty_term Q cT) \<phi> 
+    \<longleftrightarrow> wf_fmla (ty_term R cT) \<phi> \<and> vars \<phi> \<subseteq> dom Q"
+    using wf_fmla_fw wf_fmla_vars wf_fmla_bw 
     by blast
   
-  lemma wf_inst_fmla_alt: "wf_inst_fmla \<phi> \<longleftrightarrow> wf_fmla upd_inst_te (ty_inst_term Q objT) \<phi> \<and> free_vars \<phi> = {}"
-    unfolding wf_inst_fmla_def
-    using wf_inst_fmla_alt_lemma[of "(\<lambda>_. None)"]
+  lemma wf_goal_alt: "wf_goal \<phi> \<longleftrightarrow> wf_fmla (ty_term Q constT) \<phi> \<and> vars \<phi> = {}"
+    unfolding wf_goal_def
+    using wf_fmla_alt_lemma[of "(\<lambda>_. None)"]
     by simp
-  
-  lemma wf_inst_fmla_atom_corr: "wf_inst_fmla_atom f \<equiv> wf_fmla_atom (ty_inst_term (\<lambda>_. None) objT) f \<and> wf_inst_fmla f"
-    apply (induction f)
-    subgoal for x
-      apply (cases x)
-       apply auto[1]
-      subgoal for p vs
-        unfolding wf_inst_fmla_def
-        by (auto split: option.splits)
-      by auto
-    by auto
-
-  lemma wf_fmla_atom_is_wf_fmla: "wf_fmla_atom (ty_inst_term (\<lambda>_. None) objT) x \<Longrightarrow> wf_fmla upd_inst_te (ty_inst_term (\<lambda>_. None) objT) x"
-    using wf_fmla_atom_alt by auto
-
-  lemma wf_effect_inst_alt: 
-  "wf_effect_inst eff = wf_effect (ty_inst_term (\<lambda>_. None) objT) eff"
-    apply (cases eff)
-    subgoal for add del
-      apply (auto simp: wf_inst_fmla_atom_corr)[1]
-      unfolding wf_inst_fmla_def
-      by (auto intro: wf_fmla_atom_is_wf_fmla)
-    done
-
 
 end \<comment> \<open>locale \<open>ast_problem\<close>\<close>
 
@@ -1159,236 +935,25 @@ context ast_domain begin
   definition resolve_action_schema :: "name \<rightharpoonup> ast_action_schema" where
     "resolve_action_schema n = index_by ast_action_schema.name (actions D) n"
 
-  fun inst_var::"(variable \<Rightarrow> inst_term) \<Rightarrow> term \<Rightarrow> inst_term" where
-    "inst_var psubst (term.VAR x) = psubst x" 
-  | "inst_var psubst (term.CONST obj) = inst_term.OBJ obj"
+  fun subst_term where
+    "subst_term psubst (term.VAR x) = psubst x"
+  | "subst_term psubst (term.CONST c) = c"
 
-  fun cap_avoid_map::"(term \<Rightarrow> inst_term) \<Rightarrow> schematic_formula \<Rightarrow> inst_formula"
-    where
-    "cap_avoid_map f (Atom x) = Atom (map_atom f x)"
-  | "cap_avoid_map f \<bottom> = \<bottom>"
-  | "cap_avoid_map f (\<^bold>\<not>\<phi>) = \<^bold>\<not> (cap_avoid_map f \<phi>)"
-  | "cap_avoid_map f (\<phi>\<^sub>1 \<^bold>\<and> \<phi>\<^sub>2) = cap_avoid_map f \<phi>\<^sub>1 \<^bold>\<and> cap_avoid_map f \<phi>\<^sub>2"
-  | "cap_avoid_map f (\<phi>\<^sub>1 \<^bold>\<or> \<phi>\<^sub>2) = cap_avoid_map f \<phi>\<^sub>1 \<^bold>\<or> cap_avoid_map f \<phi>\<^sub>2"
-  | "cap_avoid_map f (\<phi>\<^sub>1 \<^bold>\<rightarrow> \<phi>\<^sub>2) = cap_avoid_map f \<phi>\<^sub>1 \<^bold>\<rightarrow> cap_avoid_map f \<phi>\<^sub>2"
-  | "cap_avoid_map f (\<^bold>\<exists>\<^sub>T x. \<phi>\<^sub>1) = (\<^bold>\<exists>\<^sub>T x. (cap_avoid_map (f(term.VAR x := inst_term.VAR x)) \<phi>\<^sub>1))"
-  | "cap_avoid_map f (\<^bold>\<forall>\<^sub>T x. \<phi>\<^sub>1) = (\<^bold>\<forall>\<^sub>T x. (cap_avoid_map (f(term.VAR x := inst_term.VAR x)) \<phi>\<^sub>1))"
-
-
+ text \<open>To instantiate an action schema, we first compute a substitution from
+    parameters to objects, and then apply this substitution to the
+    precondition and effect. The substitution is applied via the \<open>map_xxx\<close>
+    functions generated by the datatype package.
+    \<close>
   fun instantiate_action_schema
-    :: "ast_action_schema \<Rightarrow> object list \<Rightarrow> inst_action"
+    :: "ast_action_schema \<Rightarrow> object list \<Rightarrow> ground_action"
   where
-    "instantiate_action_schema (Action_Schema n params pre (Effect add del)) args = (let
-        tsubst = inst_var (the o (map_of (zip (map fst params) (map inst_term.OBJ args))));
-        pre_inst = cap_avoid_map tsubst pre;
-        eff_inst = Effect (map (cap_avoid_map tsubst) add) (map (cap_avoid_map tsubst) del)
+    "instantiate_action_schema (Action_Schema n params pre eff) args = (let
+        tsubst = subst_term (the o (map_of (zip (map fst params) args)));
+        pre_inst = (map_formula o map_atom) tsubst pre;
+        eff_inst = (map_ast_effect) tsubst eff
       in
-        Inst_Action pre_inst eff_inst
+        Ground_Action pre_inst eff_inst
       )"
-
-
-  lemma map_atom_maintains_vars'':
-    assumes v: "v \<in> schematic_term_atom_vars x"
-        and a: "f (term.VAR v) = inst_term.VAR v"
-      shows "v \<in> inst_term_atom_vars (map_atom f x)"
-  proof -
-    from v 
-    have "\<exists>e \<in> ent x. v \<in> schematic_term_vars e" using stav_alt by simp
-    then obtain e where
-      e: "e \<in> ent x" 
-      "v \<in> schematic_term_vars e" 
-      by auto
-    hence "e = term.VAR v"by (cases e rule: term.exhaust) auto
-    hence "f e = inst_term.VAR v" using a v by auto
-    hence "(inst_term_vars o f) e = {v}" by auto
-    with e
-    show "v \<in> inst_term_atom_vars (map_atom f x)" using itavm_alt by blast
-  qed
-
-  lemma map_atom_maintains_vars':
-    assumes v: "v \<in> schematic_term_atom_vars x"
-        and a: "\<exists>v'. f (term.VAR v) = inst_term.VAR v'"
-        and var_inst: "(\<forall>v \<in> schematic_term_atom_vars x. 
-             f (term.VAR v) = inst_term.VAR v 
-            \<or> (\<exists>obj. f(term.VAR v) = inst_term.OBJ obj))"
-      shows "v \<in> inst_term_atom_vars (map_atom f x)"
-  proof -
-    from a var_inst v
-    have "f (term.VAR v) = inst_term.VAR v" by fastforce
-    with v
-    show ?thesis using map_atom_maintains_vars'' by simp
-  qed
-  
-  lemma map_atom_maintains_vars:
-    fixes v
-    assumes a: "\<exists>v'. f (term.VAR v) = inst_term.VAR v'"
-        and var_inst: "(\<forall>v \<in> schematic_term_atom_vars x. 
-             f (term.VAR v) = inst_term.VAR v 
-            \<or> (\<exists>obj. f(term.VAR v) = inst_term.OBJ obj))"
-        and obj_inst: "\<forall>c. f (term.CONST c) = inst_term.OBJ c" 
-      shows "v \<in> schematic_term_atom_vars x \<longleftrightarrow> v \<in> inst_term_atom_vars (map_atom f x)"
-    using assms
-  proof -
-    { assume "v \<in> inst_term_atom_vars (map_atom f x)"
-      hence "\<exists>e \<in> ent x. v \<in> inst_term_vars (f e)" using itavm_alt by fastforce
-      then obtain e where
-        e: "e \<in> ent x"
-        "v \<in> inst_term_vars (f e)"
-        by auto
-      hence "f e = inst_term.VAR v" by (cases "f e") auto
-      then obtain v' where
-        v': "e = term.VAR v'" 
-        using obj_inst by (cases e) auto
-      moreover
-      hence "v' \<in> schematic_term_atom_vars x" using e stav_alt itavm_alt by fastforce
-      moreover
-      hence "e = term.VAR v" using obj_inst var_inst e v' by fastforce
-      ultimately
-      have "v \<in> schematic_term_atom_vars x"  by auto
-    }
-    with map_atom_maintains_vars' a var_inst
-    show "v \<in> schematic_term_atom_vars x \<longleftrightarrow> v \<in> inst_term_atom_vars (map_atom f x)" by blast
-  qed 
-
-  lemma cam_avoids_capture:
-    assumes "v \<in> sf_free_vars \<phi>"
-        and "f (term.VAR v) = inst_term.VAR v"
-    shows "v \<in> free_vars (cap_avoid_map f \<phi>)"
-    using assms map_atom_maintains_vars''
-    by (induction \<phi> arbitrary: f) (simp, auto)
-  
-  lemma cam_leaves_bound: 
-    assumes "v \<in> sf_bound_vars \<phi>"
-    shows "v \<in> bound_vars (cap_avoid_map f \<phi>)"
-    using assms
-    apply (induction \<phi> arbitrary: f)
-           apply auto[6]
-     apply (cases "v \<in> sf_bound_vars \<phi>")
-    using cam_avoids_capture 
-    by auto
-  
-  lemma free_is_cam_free:
-    assumes "\<exists>v'. f (term.VAR v) = inst_term.VAR v'"
-        and "\<forall>v \<in> sf_free_vars \<phi>. f (term.VAR v) = inst_term.VAR v 
-            \<or> (\<exists>obj. f(term.VAR v) = inst_term.OBJ obj)"
-        and "\<forall>c. f (term.CONST c) = inst_term.OBJ c" 
-      shows "v \<in> sf_free_vars \<phi> \<longleftrightarrow> v \<in> free_vars (cap_avoid_map f \<phi>)"
-    using assms 
-    apply (induction \<phi> arbitrary: f)
-    subgoal 1 using map_atom_maintains_vars by force
-    apply auto[5]
-    subgoal for t x
-      by (cases "x = v") auto
-    subgoal for t x
-      by (cases "x = v") auto
-    done
-  
-  lemma bound_is_cam_bound:
-    assumes var_inst: "\<forall>v \<in> sf_free_vars \<phi>. f (term.VAR v) = inst_term.VAR v 
-            \<or> (\<exists>obj. f(term.VAR v) = inst_term.OBJ obj)"
-        and obj_inst: "\<forall>c. f (term.CONST c) = inst_term.OBJ c" 
-    shows "v \<in> sf_bound_vars \<phi> \<longleftrightarrow> v \<in> bound_vars (cap_avoid_map f \<phi>)"
-    using assms
-  proof (induction \<phi> arbitrary: f)
-    case (Exists t x \<phi>)
-    have "v \<in> sf_bound_vars (\<^bold>\<exists>\<^sub>t x. \<phi>)" if a: "v \<in> bound_vars (cap_avoid_map f (\<^bold>\<exists>\<^sub>t x. \<phi>))"
-    proof (cases "v \<in> bound_vars (cap_avoid_map (f(term.VAR x := inst_term.VAR x)) \<phi>)")
-      case True
-      then show ?thesis using Exists by auto
-    next
-      case False
-      with a
-      have "v \<in> free_vars (cap_avoid_map (f(term.VAR x := inst_term.VAR x)) \<phi>) \<and> x = v" by auto
-      then show ?thesis using free_is_cam_free[of "(f(term.VAR x := inst_term.VAR x))"] Exists by fastforce
-    qed
-    thus ?case using cam_leaves_bound by blast
-  next
-    case (All t x \<phi>)
-    have "v \<in> sf_bound_vars (\<^bold>\<forall>\<^sub>t x. \<phi>)" if a: "v \<in> bound_vars (cap_avoid_map f (\<^bold>\<forall>\<^sub>t x. \<phi>))"
-    proof (cases "v \<in> bound_vars (cap_avoid_map (f(term.VAR x := inst_term.VAR x)) \<phi>)")
-      case True
-      then show ?thesis using All by auto
-    next
-      case False
-      with a
-      have "v \<in> free_vars (cap_avoid_map (f(term.VAR x := inst_term.VAR x)) \<phi>) \<and> x = v" by auto
-      then show ?thesis using free_is_cam_free[of "(f(term.VAR x := inst_term.VAR x))"] All by fastforce
-    qed
-    thus ?case using cam_leaves_bound by blast
-  qed auto
-
-  lemma map_atom_maintains_objs:
-    assumes obj: "obj \<in> schematic_term_atom_objs x"
-        and var_inst: "(\<forall>v \<in> schematic_term_atom_vars x. 
-             f (term.VAR v) = inst_term.VAR v 
-            \<or> (\<exists>obj. f(term.VAR v) = inst_term.OBJ obj))"
-        and obj_inst: "\<forall>c. f (term.CONST c) = inst_term.OBJ c" 
-      shows "obj \<in> inst_term_atom_objs (map_atom f x)"
-  proof -
-    from obj 
-    have "\<exists>e \<in> ent x. obj \<in> schematic_term_objs e" using stao_alt by simp
-    then obtain e where
-      e: "e \<in> ent x" 
-      "obj \<in> schematic_term_objs e" 
-      by auto
-    hence "e = term.CONST obj"by (cases e rule: term.exhaust) auto
-    hence "f e = inst_term.OBJ obj" using obj_inst obj by auto
-    hence "(inst_term_objs o f) e = {obj}" by auto
-    with e
-    show "obj \<in> inst_term_atom_objs (map_atom f x)" using itaom_alt by blast
-  qed
-
-  lemma assumes "obj \<in> sf_objs \<phi>"
-          and var_inst: "\<forall>v \<in> sf_free_vars \<phi>. f (term.VAR v) = inst_term.VAR v 
-              \<or> (\<exists>obj. f(term.VAR v) = inst_term.OBJ obj)"
-          and obj_inst: "\<forall>c. f (term.CONST c) = inst_term.OBJ c" 
-        shows "obj \<in> objs (cap_avoid_map f \<phi>)"
-    using assms map_atom_maintains_objs
-    by (induction \<phi> arbitrary: f) auto
-
- lemma map_atom_inst_objs:
-    assumes v: "v \<in> schematic_term_atom_vars x"
-        and f: "f (term.VAR v) = inst_term.OBJ obj"
-      shows "obj \<in> inst_term_atom_objs (map_atom f x)"
-  proof -
-    from v
-    have "\<exists>e \<in> ent x. v \<in> schematic_term_vars e" using stav_alt by simp
-    then obtain e where
-      e: "e \<in> ent x" 
-      "v \<in> schematic_term_vars e" 
-      by auto
-    hence "e = term.VAR v" by (cases e rule: term.exhaust) auto
-    hence "f e = inst_term.OBJ obj" using f by auto
-    hence "(inst_term_objs o f) e = {obj}" by auto
-    with e
-    show "obj \<in> inst_term_atom_objs (map_atom f x)" using itaom_alt by blast
-  qed
-
-  lemma cam_introduces_objs:
-      assumes "v \<in> sf_free_vars \<phi>"
-          and "f (term.VAR v) = inst_term.OBJ obj"
-        shows "obj \<in> objs (cap_avoid_map f \<phi>)"
-    using assms map_atom_inst_objs
-    apply (induction \<phi> arbitrary: f)
-           apply auto
-    done
-
-  lemma cam_instantiates_correctly:
-    assumes "v \<in> sf_free_vars \<phi>"
-        and "\<forall>v \<in> sf_free_vars \<phi>. f (term.VAR v) = inst_term.VAR v 
-            \<or> (\<exists>obj. f(term.VAR v) = inst_term.OBJ obj)"
-        and "\<forall>c. f (term.CONST c) = inst_term.OBJ c" 
-      shows "v \<in> free_vars (cap_avoid_map f \<phi>) \<or> (\<exists>obj. f(term.VAR v) = inst_term.OBJ obj \<and> obj \<in> objs (cap_avoid_map f \<phi>))"
-    using assms cam_introduces_objs cam_avoids_capture
-    by blast
-
-  lemma cam_instantiates_fv_to_obj:
-    assumes "v \<in> sf_free_vars \<phi>"
-        and "\<forall>v \<in> sf_free_vars \<phi>. (\<exists>obj. f(term.VAR v) = inst_term.OBJ obj)"
-        and "\<forall>c. f (term.CONST c) = inst_term.OBJ c" 
-      shows "(\<exists>obj. f(term.VAR v) = inst_term.OBJ obj \<and> obj \<in> objs (cap_avoid_map f \<phi>))"
-    using assms cam_introduces_objs 
-    by blast
 
 end \<comment> \<open>Context of \<open>ast_domain\<close>\<close>
 
@@ -1400,7 +965,7 @@ context ast_problem begin
     "I \<equiv> set (init P)"
 
   text \<open>Resolve a plan action and instantiate the referenced action schema.\<close>
-  fun resolve_instantiate :: "plan_action \<Rightarrow> inst_action" where
+  fun resolve_instantiate :: "plan_action \<Rightarrow> ground_action" where
     "resolve_instantiate (PAction n args) =
       instantiate_action_schema
         (the (resolve_action_schema n))
@@ -1443,7 +1008,7 @@ context ast_problem begin
         )"
   text \<open>
     TODO: The second conjunct is redundant, as instantiating a well formed
-      action with valid objects yields a valid effect.
+      action with valid objects yield a valid effect.
   \<close>
 
 
@@ -1455,13 +1020,18 @@ context ast_problem begin
   where
     "plan_action_path M \<pi>s M' =
         ((\<forall>\<pi> \<in> set \<pi>s. wf_plan_action \<pi>)
-      \<and> inst_action_path M (map resolve_instantiate \<pi>s) M')"
-                                              
+      \<and> ground_action_path M (map resolve_instantiate \<pi>s) M')"
+
+  text \<open>Instantiation of a goal\<close>
+  fun inst_goal::"schematic_formula \<Rightarrow> ground_formula" where
+  "inst_goal \<phi> = (let tsubst = subst_term (the o (Map.empty))
+        in (map_formula o map_atom) tsubst \<phi>)"                           
+  
   text \<open>A plan is valid wrt.\ a given initial model, if it forms a path to a
     goal model \<close>
   definition valid_plan_from :: "world_model \<Rightarrow> plan \<Rightarrow> bool" where
-    "valid_plan_from M \<pi>s = (\<exists>M'. plan_action_path M \<pi>s M' \<and> M' \<^sup>c\<TTurnstile>\<^sub>= (goal P))"
-
+    "valid_plan_from M \<pi>s = (\<exists>M'. plan_action_path M \<pi>s M' \<and> M' \<^sup>c\<TTurnstile>\<^sub>= inst_goal (goal P))"
+  (* instantiate the goal wrt nothing *)
   (* Implementation note: resolve and instantiate already done inside
       enabledness check, redundancy! *)
 
@@ -1471,7 +1041,7 @@ context ast_problem begin
     where "valid_plan \<equiv> valid_plan_from I"
 
   text \<open>Concise definition used in paper:\<close>
-  lemma "valid_plan \<pi>s \<equiv> \<exists>M'. plan_action_path I \<pi>s M' \<and> M' \<^sup>c\<TTurnstile>\<^sub>= (goal P)"
+  lemma "valid_plan \<pi>s \<equiv> \<exists>M'. plan_action_path I \<pi>s M' \<and> M' \<^sup>c\<TTurnstile>\<^sub>= inst_goal (goal P)"
     unfolding valid_plan_def valid_plan_from_def by auto
 
 
@@ -1492,10 +1062,10 @@ context ast_problem begin
     executing the action instance, it is natural to define a well-formedness
     concept for action instances.\<close>
 
-  fun wf_inst_action :: "inst_action \<Rightarrow> bool" where
-    "wf_inst_action (Inst_Action pre eff) \<longleftrightarrow> (
-        wf_inst_fmla pre   
-      \<and> wf_effect (ty_inst_term (\<lambda>_. None) objT) eff
+  fun wf_ground_action :: "ground_action \<Rightarrow> bool" where
+    "wf_ground_action (Ground_Action pre eff) \<longleftrightarrow> (
+        wf_fmla objT pre
+      \<and> wf_effect objT eff
       )
     "
 
@@ -1546,10 +1116,10 @@ context ast_problem begin
     by (simp_all add: constT_ss_objT)
 
   context
-    fixes Q S and f :: "variable \<Rightarrow> inst_term"
-    assumes INST: "is_of_type Q x T \<Longrightarrow> is_of_type (ty_inst_term (Q |` S) objT) (f x) T"
-  begin 
-    
+    fixes Q and f :: "variable \<Rightarrow> object"
+    assumes INST: "is_of_type Q x T \<Longrightarrow> is_of_type objT (f x) T"
+  begin
+
     lemma is_of_type_var_conv: "is_of_type (ty_term Q objT) (term.VAR x) T  \<longleftrightarrow> is_of_type Q x T"
       unfolding is_of_type_def by (auto)
 
@@ -1557,39 +1127,24 @@ context ast_problem begin
       unfolding is_of_type_def
       by (auto split: option.split)
 
-    lemma INST': "is_of_type (ty_term Q objT) x T \<Longrightarrow> is_of_type (ty_inst_term (Q |` S) objT) (inst_var f x) T"
-      apply (cases x) using INST 
-      apply auto[1]
-       apply (simp add: ast_domain.is_of_type_def)
-      by (simp add: is_of_type_def)
+    lemma INST': "is_of_type (ty_term Q objT) x T \<Longrightarrow> is_of_type objT (subst_term f x) T"
+      apply (cases x) using INST apply (auto simp: is_of_type_var_conv is_of_type_const_conv)
+      done
 
-    lemma wf_inst_eq_aux: "Q x = Some T \<Longrightarrow> ty_inst_term (Q |` S) objT (f x) \<noteq> None"
+
+    lemma wf_inst_eq_aux: "Q x = Some T \<Longrightarrow> objT (f x) \<noteq> None"
       using INST[of x T] unfolding is_of_type_def
       by (auto split: option.splits)
 
-    lemma wf_inst_eq_aux1: "Q x = Some T \<Longrightarrow>\<exists>T'. ty_inst_term (Q |` S) objT (f x) = Some T' \<and> of_type T' T"
-    proof -
-      assume "Q x = Some T"
-      hence "is_of_type Q x T" unfolding is_of_type_def by simp
-      from this[THEN INST] have "is_of_type (ty_inst_term (Q |` S) objT) (f x) T" .
-      then obtain T' where
-        "ty_inst_term (Q |` S) objT (f x) = Some T'" 
-        "of_type T' T"
-        unfolding is_of_type_def
-        by (auto split: option.splits)
-      thus ?thesis
-        by auto
-    qed
+    lemma wf_inst_eq_aux': "ty_term Q objT x = Some T \<Longrightarrow> objT (subst_term f x) \<noteq> None"
+      by (cases x) (auto simp: wf_inst_eq_aux)
 
-    lemma wf_inst_eq_aux': "ty_term Q objT x = Some T \<Longrightarrow> ty_inst_term (Q |` S) objT (inst_var f x) \<noteq> None"
-      apply (cases x) 
-      by (auto simp: wf_inst_eq_aux split: option.split)
 
     lemma wf_inst_atom:
       assumes "wf_atom (ty_term Q constT) a"
-      shows "wf_atom (ty_inst_term (Q |` S) objT) ((map_atom o inst_var) f a)"
+      shows "wf_atom objT (map_atom (subst_term f) a)"
     proof -
-      have X1: "list_all2 (is_of_type (ty_inst_term (Q |` S) objT)) (map (inst_var f) xs) Ts" if
+      have X1: "list_all2 (is_of_type objT) (map (subst_term f) xs) Ts" if
         "list_all2 (is_of_type (ty_term Q objT)) xs Ts" for xs Ts
         using that
         apply induction
@@ -1598,295 +1153,75 @@ context ast_problem begin
       then show ?thesis
         using assms[THEN wf_atom_constT_imp_objT] wf_inst_eq_aux'
         by (cases a; auto split: option.splits)
+
     qed
 
     lemma wf_inst_formula_atom:
       assumes "wf_fmla_atom (ty_term Q constT) a"
-      shows "wf_fmla_atom (ty_inst_term (Q |` S) objT) ((cap_avoid_map o inst_var) f a)"
+      shows "wf_fmla_atom objT ((map_formula o map_atom o subst_term) f a)"
       using assms[THEN wf_fmla_atom_constT_imp_objT] wf_inst_atom
-      apply (cases "((ty_term Q constT), a)" rule: wf_fmla_atom.cases; auto split: option.splits)
+      apply (cases a rule: wf_fmla_atom.cases; auto split: option.splits)
       by (simp add: INST' list.rel_map(1) list_all2_mono)
 
-    lemma wf_inst_effect_aux:
-      assumes "wf_effect (ty_term Q constT) (Effect add del)"
-      shows "wf_effect (ty_inst_term (Q |` S) objT) (Effect ((map o cap_avoid_map o inst_var) f add) ((map o cap_avoid_map o inst_var) f del))"
+    lemma wf_inst_effect:
+      assumes "wf_effect (ty_term Q constT) \<phi>"
+      shows "wf_effect objT ((map_ast_effect o subst_term) f \<phi>)"
       using assms
-      proof (induction "(Effect add del)")
-        case (Effect)
+      proof (induction \<phi>)
+        case (Effect x1a x2a)
         then show ?case using wf_inst_formula_atom by auto
       qed
-end
 
-  lemma f'_maintains_type:
-    fixes v T
-    assumes a: "is_of_type (Q(v\<mapsto>ty)) x T"
-        and f': "f' = f(v := inst_term.VAR v)"
-        and S': "S' = {x. \<exists>x'. x \<in> dom (Q(v\<mapsto>ty)) \<and> f' x = inst_term.VAR x'}"
-        and S:  "S = {x. \<exists>x'. x \<in> dom Q \<and> f x = inst_term.VAR x'}"
-        and INST: "\<And>x T. is_of_type Q x T \<Longrightarrow> is_of_type (ty_inst_term (Q |` S) objT) (f x) T"
-        and inv: "\<And>v v'. v \<in> dom Q \<Longrightarrow> f v = inst_term.VAR v' \<Longrightarrow> v = v'"
-      shows "is_of_type (ty_inst_term (Q(v\<mapsto>ty) |` S') objT) (f' x) T"
-    using assms
+    lemma wf_inst_formula:
+      assumes "wf_fmla (ty_term Q constT) \<phi>"
+      shows "wf_fmla objT ((map_formula o map_atom o subst_term) f \<phi>)"
+      using assms
+      by (induction \<phi>) (auto simp: wf_inst_atom dest: wf_inst_eq_aux)
+
+  end
+
+  text \<open>Instantiating a well-formed goal will result in a well-formed formula\<close>
+  theorem wf_instantiate_goal:
+    assumes "wf_goal \<phi>"
+    shows "wf_fmla objT (inst_goal \<phi>)"
   proof -
-    fix v T
-    assume a:  "is_of_type (Q(v\<mapsto>ty)) x T"
-    assume f': "f' = f(v := inst_term.VAR v)"
-    assume S': "S' = {x. \<exists>x'. x \<in> dom (Q(v\<mapsto>ty)) \<and> f' x = inst_term.VAR x'}"
-    show "is_of_type (ty_inst_term (Q(v\<mapsto>ty) |` S') objT) (f' x) T"
-    proof (cases "v = x")
-      case v: True
-      with a
-      have "(Q(v\<mapsto>ty)) v = Some ty \<and> of_type ty T"
-        unfolding is_of_type_def by auto
-      moreover
-      have "v \<in> S'" using S' f' by auto
-      ultimately 
-      have "(Q(v\<mapsto>ty) |` S') v = Some ty \<and> of_type ty T" by auto
-      hence "is_of_type (ty_inst_term (Q(v\<mapsto>ty) |` S') objT) (inst_term.VAR v) T"
-        unfolding is_of_type_def by simp
-      moreover 
-      have "inst_term.VAR v = f' x" using v f' by auto
-      ultimately 
-      show "is_of_type (ty_inst_term (Q(v\<mapsto>ty) |` S') objT) (f' x) T"
-        by simp
-    next
-      case v: False
-      obtain xt where
-        x': "(Q(v\<mapsto>ty)) x  = Some xt \<and> of_type xt T" 
-        using a
-        unfolding is_of_type_def
-        by (auto split: option.splits)
-      
-      have "Q x = Some xt \<and> of_type xt T" using v x' by auto
-      hence "is_of_type Q x T" unfolding is_of_type_def by auto
-      from INST[OF this]
-      have inst_term_start: "is_of_type (ty_inst_term (Q |` S) objT) (f x) T " .
-
-      show ?thesis  
-      proof (cases "f x" rule: inst_term.exhaust)
-        case (OBJ obj')
-        with inst_term_start
-        have "is_of_type (ty_inst_term (Q |` S) objT) (inst_term.OBJ obj') T" by auto
-        hence "is_of_type objT obj' T" unfolding is_of_type_def by auto
-        hence "is_of_type (ty_inst_term (Q(v\<mapsto>ty) |` S') objT) (inst_term.OBJ obj') T" unfolding is_of_type_def by auto
-        thus ?thesis using OBJ f' v by auto
-      next
-        case (VAR v')
-        with inst_term_start
-        have "is_of_type (ty_inst_term (Q |` S) objT) (inst_term.VAR v') T" by auto
-        hence iQS: "is_of_type (Q |` S) v' T" unfolding is_of_type_def by auto
-        hence "\<exists>xt'. (Q |` S) v' = Some xt'" unfolding is_of_type_def using case_optionE by blast
-        hence "v' \<in> S" by (simp add: restrict_map_eq(2))
-        with S' f' VAR 
-        have "v' \<in> S'" using S by auto
-        from  iQS \<open>v' \<in> S\<close> 
-        have "is_of_type Q v' T" by (simp add: is_of_type_def)
-        hence "is_of_type (Q(v\<mapsto>ty)) v' T" using v a VAR inv \<open>Q x = Some xt \<and> of_type xt T\<close> by blast 
-        hence "is_of_type (Q(v\<mapsto>ty) |` S') v' T" using \<open>v' \<in> S'\<close> unfolding is_of_type_def using restrict_in by metis
-        hence "is_of_type (ty_inst_term (Q(v \<mapsto> ty) |` S') objT) (inst_term.VAR v') T" unfolding is_of_type_def by auto
-        moreover 
-        have "f' x = f x" using f' v by simp
-        ultimately 
-        show ?thesis using VAR by auto
-      qed
-    qed
-  qed 
-
-
-  lemma wf_inst_formula_aux:
-    assumes "wf_fmla upd_te (ty_term Q constT) \<phi>"
-        and "S = {x. \<exists>x'. x \<in> dom Q \<and>  f x = inst_term.VAR x'}"
-        and "\<And>x T. is_of_type Q x T \<Longrightarrow> is_of_type (ty_inst_term (Q |` S) objT) (f x) T"
-        and "\<And>v v'. v \<in> dom Q \<Longrightarrow> f v = inst_term.VAR v' \<Longrightarrow> v = v'"
-    shows "wf_fmla upd_inst_te (ty_inst_term (Q |` S) objT) ((cap_avoid_map o inst_var) f \<phi>)"
-  using assms
-  proof (induction \<phi> arbitrary: Q f S)
-    case (Atom x)
-    hence 1: "wf_atom (ty_term Q constT) x" by auto
-    with wf_inst_atom[of Q S f x] Atom(3) 
-    have "wf_atom (ty_inst_term (Q |` S) objT) ((map_atom o inst_var) f x)" by blast
-    hence "wf_fmla upd_inst_te (ty_inst_term (Q |` S) objT) ((cap_avoid_map o inst_var) f (Atom x))" by auto
-    then show ?case unfolding wf_inst_fmla_def 
-      using 1 Atom(1) by auto
-  next
-    case (Exists t v \<phi>)
-    thm Exists.prems
-    have "wf_fmla upd_te (ty_term (Q(v\<mapsto>t)) constT) \<phi>" using ty_term_upd Exists.prems(1) by simp
-    moreover
-    obtain S' f' where 
-          S': "S' = {x. \<exists>x'. x \<in> dom (Q(v\<mapsto>t)) \<and> f' x = inst_term.VAR x'}"
-      and f': "f' = f(v := inst_term.VAR v)"
-      by auto
-    moreover
-    with Exists.prems(2)
-    have S'_def: "S'= insert v S"  by auto
-    moreover
-    from Exists.prems
-    have "\<And>x T. is_of_type (Q(v\<mapsto>t)) x T \<Longrightarrow> is_of_type (ty_inst_term (Q(v\<mapsto>t) |` S') objT) (f' x) T"
-      using f'_maintains_type[OF _ f' S'] by blast
-    moreover 
-    from Exists.prems(4) f'
-    have "\<And>x x'. x \<in> dom (Q(v\<mapsto>t)) \<Longrightarrow> f' x = inst_term.VAR x' \<Longrightarrow> x = x'"
-      subgoal for x1 x2
-        by (cases "x1 = v") auto
-      done
-    ultimately
-    have "wf_fmla upd_inst_te (ty_inst_term (Q(v\<mapsto>t) |` (S')) objT) ((cap_avoid_map \<circ> inst_var) f' \<phi>)"
-      using Exists.IH by blast 
-    hence "wf_fmla upd_inst_te (ty_inst_term ((Q |` S) (v\<mapsto>t)) objT) ((cap_avoid_map \<circ> inst_var) f' \<phi>)"
-      using S'_def restrict_map_upd 
-      by metis
-    hence "wf_fmla upd_inst_te (upd_inst_te (ty_inst_term ((Q |` S) (v\<mapsto>t)) objT) v t) ((cap_avoid_map \<circ> inst_var) f' \<phi>)"
-      using ty_inst_term_upd by force
-    moreover
-    have "inst_var f' = (inst_var f)(term.VAR v := inst_term.VAR v)"
-      apply (subst f', rule ext)
-      subgoal for x
-        by (cases x) auto
-      done
-    hence "cap_avoid_map (inst_var f') = cap_avoid_map ((inst_var f)(term.VAR v := inst_term.VAR v))"
-      by simp
-    hence "(cap_avoid_map \<circ> inst_var) f (\<^bold>\<exists>\<^sub>t v. \<phi>) = (\<^bold>\<exists>\<^sub>t v. ((cap_avoid_map \<circ> inst_var) f' \<phi>))"
-      using f' by simp
-    ultimately
-    show "wf_fmla upd_inst_te (ty_inst_term (Q |` S) objT) ((cap_avoid_map \<circ> inst_var) f (\<^bold>\<exists>\<^sub>t v. \<phi>))"
-      using f' ty_inst_term_upd by auto
-  next
-    case (All t v \<phi>)
-    hence "wf_fmla upd_te (ty_term (Q(v\<mapsto>t)) constT) \<phi>" using ty_term_upd by auto
-    moreover
-    obtain S' f' where 
-          S': "S' = {x. \<exists>x'. x \<in> dom (Q(v\<mapsto>t)) \<and> f' x = inst_term.VAR x'}"
-      and f': "f' = f(v := inst_term.VAR v)"
-      by auto
-    moreover
-    hence S'_def: "S'= insert v S" using All.prems(2) by auto
-    moreover
-    have "\<And>x T. is_of_type (Q(v\<mapsto>t)) x T \<Longrightarrow> is_of_type (ty_inst_term (Q(v\<mapsto>t) |` S') objT) (f' x) T"
-      using f'_maintains_type[OF _ f' S' ] All.prems by blast
-    moreover 
-    from All.prems(4) f'
-    have "\<And>x x'. x \<in> dom (Q(v\<mapsto>t)) \<Longrightarrow> f' x = inst_term.VAR x' \<Longrightarrow> x = x'"
-      subgoal for x1 x2
-        by (cases "x1 = v") auto
-      done
-    ultimately
-    have "wf_fmla upd_inst_te (ty_inst_term (Q(v\<mapsto>t) |` (S')) objT) ((cap_avoid_map \<circ> inst_var) f' \<phi>)"
-      using All.IH by blast 
-    hence "wf_fmla upd_inst_te (ty_inst_term ((Q |` S) (v\<mapsto>t)) objT) ((cap_avoid_map \<circ> inst_var) f' \<phi>)"
-      using S'_def restrict_map_upd 
-      by metis
-    hence "wf_fmla upd_inst_te (upd_inst_te (ty_inst_term ((Q |` S) (v\<mapsto>t)) objT) v t) ((cap_avoid_map \<circ> inst_var) f' \<phi>)"
-      using ty_inst_term_upd by force
-    moreover
-    have "inst_var f' = (inst_var f)(term.VAR v := inst_term.VAR v)"
-      apply (subst f', rule ext)
-      subgoal for x
-        by (cases x) auto
-      done
-    hence "cap_avoid_map (inst_var f') = cap_avoid_map ((inst_var f)(term.VAR v := inst_term.VAR v))"
-      by simp
-    hence "(cap_avoid_map \<circ> inst_var) f (\<^bold>\<forall>\<^sub>t v. \<phi>) = (\<^bold>\<forall>\<^sub>t v. ((cap_avoid_map \<circ> inst_var) f' \<phi>))"
-      using f' by simp
-    ultimately
-    show "wf_fmla upd_inst_te (ty_inst_term (Q |` S) objT) ((cap_avoid_map \<circ> inst_var) f (\<^bold>\<forall>\<^sub>t v. \<phi>))"
-      using f' ty_inst_term_upd by auto
-  qed auto
-
-  lemma full_inst_imp_dom_empty:
-    assumes INST: "\<And>x T. is_of_type Q x T \<Longrightarrow> is_of_type (ty_inst_term (\<lambda>_. None) objT) (f x) T"
-        and inv:  "\<And>v x. x \<in> dom Q \<Longrightarrow> f x = inst_term.VAR v \<Longrightarrow> x = v"
-      shows "{x. \<exists>x'. x \<in> dom Q \<and> f x = inst_term.VAR x'} = {}"
-    using assms
-  proof -
-    have "\<exists>obj. f x = inst_term.OBJ obj" 
-      if "x \<in> dom Q" for x 
-      using that
-    proof -
-      assume "x \<in> dom Q"
-      then obtain T where
-        "is_of_type Q x T"
-        unfolding is_of_type_def by fastforce
-      with INST
-      have "is_of_type (ty_inst_term (\<lambda>_. None) objT) (f x) T"
-        by blast
-      then obtain vT where
-        "ty_inst_term (\<lambda>_. None) objT (f x) = Some vT \<and> of_type vT T" 
-        unfolding is_of_type_def by (auto split: option.splits)
-      thus "\<exists>obj. f x = inst_term.OBJ obj"
-        by (cases "f x") auto
-    qed
-    thus "{x. \<exists>x'. x \<in> dom Q \<and> f x = inst_term.VAR x'} = {}" by force
-  qed
-
-  lemma wf_inst_formula:
-    assumes wff:  "wf_fmla upd_te (ty_term Q constT) \<phi>"
-        and INST: "\<And>x T. is_of_type Q x T \<Longrightarrow> is_of_type (ty_inst_term (\<lambda>_. None) objT) (f x) T"
-        and inv:  "\<And>v x. x \<in> dom Q \<Longrightarrow> f x = inst_term.VAR v \<Longrightarrow> x = v"
-      shows "wf_inst_fmla ((cap_avoid_map o inst_var) f \<phi>)"
-  proof -
-    have S: "{} = {x. \<exists>x'. x \<in> dom Q \<and> f x = inst_term.VAR x'}" 
-      using full_inst_imp_dom_empty[OF INST inv] by presburger
-    
-    with INST
-    have "\<And>x T. is_of_type Q x T \<Longrightarrow> is_of_type (ty_inst_term (Q |` {}) objT) (f x) T" by auto
-    
-    from wf_inst_formula_aux[OF wff S this inv]
-    have "wf_fmla upd_inst_te (ty_inst_term (Q |` {}) objT) ((cap_avoid_map o inst_var) f \<phi>)" by presburger
-    hence "wf_fmla upd_inst_te (ty_inst_term (\<lambda>_. None) objT) ((cap_avoid_map o inst_var) f \<phi>)"using restrict_map_to_empty[of Q] by argo
-    thus "wf_inst_fmla ((cap_avoid_map o inst_var) f \<phi>)" unfolding wf_inst_fmla_def by simp
-  qed 
-
-  lemma wf_inst_effect:
-    fixes add::"schematic_formula list" and del::"schematic_formula list" and f
-    assumes "wf_effect (ty_term Q constT) (Effect add del)"
-      and INST: "\<And>x T. is_of_type Q x T \<Longrightarrow> is_of_type (ty_inst_term (\<lambda>_. None) objT) (f x) T"
-      and inv:  "\<And>v x. x \<in> dom Q \<Longrightarrow> f x = inst_term.VAR v \<Longrightarrow> x = v"
-    shows "wf_effect (ty_inst_term (\<lambda>_.None) objT) (Effect ((map o cap_avoid_map o inst_var) f add) ((map o cap_avoid_map o inst_var) f del))"
-    using assms
-  proof -
-    assume a: "wf_effect (ty_term Q constT) (Effect add del)"
-    have S: "{} = {x. \<exists>x'. x \<in> dom Q \<and> f x = inst_term.VAR x'}" 
-      using full_inst_imp_dom_empty[OF INST inv] by presburger
-
-    with INST
-    have INST': "\<And>x T. is_of_type Q x T \<Longrightarrow> is_of_type (ty_inst_term (Q |` {}) objT) (f x) T" by auto
-
-    from wf_inst_effect_aux[OF this a]
-    have "wf_effect (ty_inst_term (Q |` {}) objT) 
-                  (Effect ((map o cap_avoid_map o inst_var) f add) 
-                          ((map o cap_avoid_map o inst_var) f del))" 
-      by presburger
-
-    thus "wf_effect (ty_inst_term (\<lambda>_. None) objT) 
-                  (Effect ((map o cap_avoid_map o inst_var) f add) 
-                          ((map o cap_avoid_map o inst_var) f del))" 
-      using restrict_map_to_empty[of Q] by argo
+    have INST: "is_of_type objT ((the \<circ> Map.empty) x) T"
+      if "is_of_type (Map.empty) x T" for x T
+      using that 
+      unfolding is_of_type_def
+      by (auto split: option.splits)
+    with assms
+    show ?thesis
+      using wf_inst_formula
+      unfolding wf_goal_def
+      by (fastforce split: term.splits simp: Let_def comp_apply[abs_def])
   qed
 
 
-  
   text \<open>Instantiating a well-formed action schema with compatible arguments
     will yield a well-formed action instance.
   \<close>
   theorem wf_instantiate_action_schema:
     assumes "action_params_match a args"
     assumes "wf_action_schema a"
-    shows "wf_inst_action (instantiate_action_schema a args)"
+    shows "wf_ground_action (instantiate_action_schema a args)"
   proof (cases a)
     case [simp]: (Action_Schema name params pre eff)
-    let ?f = "the o (map_of (zip (map fst params) (map inst_term.OBJ args)))"
-    
-    have INST: "is_of_type (ty_inst_term (\<lambda>_. None) objT) (?f x) T"
+    have INST:
+      "is_of_type objT ((the \<circ> map_of (zip (map fst params) args)) x) T"
       if "is_of_type (map_of params) x T" for x T
       using that
       apply (rule is_of_type_map_ofE)
       using assms
       apply (clarsimp simp: Let_def)
+        apply (thin_tac "wf_fmla (ty_term (map_of params) constT) pre")
+        apply (thin_tac "wf_effect (ty_term (map_of params) constT) eff")
       subgoal for i xT
         unfolding action_params_match_def
+        thm lookup_zip_idx_eq
         apply (subst lookup_zip_idx_eq[where i=i];
           (clarsimp simp: list_all2_lengthD)?)
+        thm list_all2_nthD2
         apply (frule list_all2_nthD2[where p=i]; simp?)
         apply (auto
                 simp: is_obj_of_type_alt is_of_type_def
@@ -1894,238 +1229,11 @@ end
                 split: option.splits)
         done
       done
-
-    have inv:   "x = v" 
-      if  d:    "x \<in> dom (map_of params)" 
-      and asmt: "?f x = inst_term.VAR v" 
-    for x v
-      using that
-      apply (subst (asm) dom_map_of_conv_image_fst, subst (asm) sym[OF set_map], subst (asm) in_set_conv_nth)
-      using assms
-      unfolding action_params_match_def
-      apply (clarsimp simp: Let_def)
-      subgoal for i
-        apply (drule list_all2_lengthD)
-        apply (subst (asm) lookup_zip_idx_eq)
-        by auto
-      done
-
-    have "wf_fmla upd_te (ty_term (map_of params) constT) pre" 
-      using assms by (auto simp: Let_def)
-    with INST inv
-    have inst_pre: "wf_inst_fmla ((cap_avoid_map o inst_var) ?f pre)" 
-      using wf_inst_formula by blast
-
-    obtain add del where
-      eff: "eff = Effect add del"
-      by (cases rule: ast_effect.exhaust)
-    with assms
-    have "wf_effect (ty_term (map_of params) constT) (Effect add del)"
-      by (auto simp: Let_def)
-    with INST inv
-    have inst_eff: "wf_effect (ty_inst_term (\<lambda>_.None) objT)
-        (Effect ((map o cap_avoid_map o inst_var) ?f add) 
-                ((map o cap_avoid_map o inst_var) ?f del))"
-      using wf_inst_effect by blast
-
-    from inst_pre eff inst_eff
-    show "wf_inst_action (instantiate_action_schema a args)"
-      by (simp add: Let_def)
+    then show ?thesis
+      using assms(2) wf_inst_formula wf_inst_effect
+      by (fastforce split: term.splits simp: Let_def comp_apply[abs_def])
   qed
-
-  corollary inst_maintains_bound:
-    assumes a[simp]: "a = Action_Schema n params pre (Effect add del)"
-        and match:"action_params_match a args"
-        and wf: "wf_action_schema a"
-        and inst: "Inst_Action pre' (Effect add' del') = instantiate_action_schema a args"
-      shows "sf_bound_vars pre = bound_vars pre' 
-            \<and> (\<forall>i < length add. sf_bound_vars (add ! i) = bound_vars (add' ! i))
-            \<and> (\<forall>i < length del. sf_bound_vars (del ! i) = bound_vars (del' ! i))"
-  proof -
-    let ?f = "inst_var (the o (map_of (zip (map fst params) (map inst_term.OBJ args))))"
-
-    have well_inst:
-     "\<forall>v. v \<in> sf_bound_vars \<phi> \<longleftrightarrow> v \<in> bound_vars (cap_avoid_map ?f \<phi>)"
-      if "wf_fmla upd_te (ty_term (map_of params) constT) \<phi>"
-        for \<phi> 
-    proof -
-      from that 
-      have  "sf_free_vars \<phi> \<subseteq> dom (map_of params)" 
-        using wf_schematic_fmla_free_vars[of "map_of params"]
-        by force
-      hence "sf_free_vars \<phi> \<subseteq> set (map fst params)"
-        by (simp add: dom_map_of_conv_image_fst)
-      moreover
-      from match
-      have "length params = length args"
-        unfolding action_params_match_def using list_all2_lengthD by fastforce
-      hence "length (map fst params) = length (map inst_term.OBJ args)"
-        by fastforce
-      hence "\<forall>v \<in> set (map fst params).(\<exists>obj. (map_of (zip (map fst params) (map inst_term.OBJ args))) v = Some (inst_term.OBJ obj))"
-        find_theorems name: "map_of_zip"
-        apply -
-        apply (rule ballI)
-        subgoal for v
-          apply (drule map_of_zip_is_Some)
-          apply auto[1]
-          apply (drule map_of_SomeD)
-          apply (erule in_set_zipE)
-          by auto
-        done
-      ultimately
-      have "\<forall>v \<in> sf_free_vars \<phi>.(\<exists>obj. (the o (map_of (zip (map fst params) (map inst_term.OBJ args)))) v = inst_term.OBJ obj)"
-        by fastforce
-      hence "\<forall>v \<in> sf_free_vars \<phi>.(\<exists>obj. ?f (term.VAR v) = inst_term.OBJ obj)"
-        by simp
-      thus "\<forall>v. v \<in> sf_bound_vars \<phi> \<longleftrightarrow> v \<in> bound_vars (cap_avoid_map ?f \<phi>)"
-        using bound_is_cam_bound
-        by simp
-    qed
-    
-    have "sf_bound_vars pre = bound_vars pre'" using inst wf well_inst by (auto simp: Let_def)
-    moreover
-    have "sf_bound_vars (add ! i) = bound_vars (add' ! i)" 
-      if "i < length add" for i
-    proof -
-      have "wf_fmla_atom (ty_term (map_of params) constT) (add ! i)" 
-        using wf that by (auto simp: Let_def)
-      hence "wf_fmla upd_te (ty_term (map_of params) constT) (add ! i)" 
-        using wf_fmla_atom_alt by blast
-      moreover have "add' ! i = cap_avoid_map ?f (add ! i)" using inst that by (auto simp: Let_def)
-      ultimately show "sf_bound_vars (add ! i) = bound_vars (add' ! i)"
-        using well_inst by auto
-    qed
-    moreover
-    have "sf_bound_vars (del ! i) = bound_vars (del' ! i)" 
-      if "i < length del" for i
-    proof -
-      have "wf_fmla_atom (ty_term (map_of params) constT) (del ! i)" 
-        using wf that by (auto simp: Let_def)
-      hence "wf_fmla upd_te (ty_term (map_of params) constT) (del ! i)" 
-        using wf_fmla_atom_alt by blast
-      moreover have "del' ! i = cap_avoid_map ?f (del ! i)" using inst that by (auto simp: Let_def)
-      ultimately show "sf_bound_vars (del ! i) = bound_vars (del' ! i)"
-        using well_inst by auto
-    qed
-    ultimately show ?thesis by simp
-  qed
-  
-  corollary inst_leaves_no_free_vars:
-    assumes match:"action_params_match a args"
-          and wf: "wf_action_schema a"
-          and inst: "Inst_Action pre' (Effect add' del') = instantiate_action_schema a args"
-        shows "free_vars pre' = {} 
-              \<and> (\<forall>a \<in> set add'. free_vars a = {})
-              \<and> (\<forall>d \<in> set del'. free_vars d = {})"
-  proof -
-    from wf_instantiate_action_schema[OF match wf] inst
-    have 1: "wf_inst_action (Inst_Action pre' (Effect add' del'))" by auto
-    hence "wf_inst_fmla pre'" by fastforce
-    hence "free_vars pre' = {}" using wf_inst_fmla_alt by blast
-    moreover
-    from 1
-    have "\<forall>a \<in> set add'. wf_inst_fmla a"
-      using wf_fmla_atom_alt unfolding wf_inst_fmla_def
-      by auto
-    hence "\<forall>a \<in> set add'. free_vars a = {}" using wf_inst_fmla_alt by blast
-    moreover
-    from 1
-    have "\<forall>d \<in> set del'. wf_inst_fmla d"
-      using wf_fmla_atom_alt wf_inst_fmla_def unfolding wf_inst_fmla_def
-      by fastforce
-    hence "\<forall>d \<in> set del'. free_vars d = {}" using wf_inst_fmla_alt by blast
-    ultimately
-    show ?thesis by simp
-  qed
-
-  term "\<forall>x. (\<exists>x. VAR y \<or> VAR x) \<and> VAR x"
-  
-  corollary inst_maps_fv_to_obj:
-    assumes a[simp]: "a = Action_Schema n params pre (Effect add del)"
-        and match:"action_params_match a args"
-        and wf: "wf_action_schema a"
-        and inst: "Inst_Action pre' (Effect add' del') = instantiate_action_schema a args"
-        and f[simp]: "f = inst_var (the o (map_of (zip (map fst params) (map inst_term.OBJ args))))"
-      shows "\<forall>v \<in> sf_free_vars pre. (\<exists>obj. f (term.VAR v) = inst_term.OBJ obj \<and> obj \<in> objs pre') 
-            \<and> (\<forall>i < length add. \<forall>v \<in> sf_free_vars (add ! i). (\<exists>obj. f (term.VAR v) = inst_term.OBJ obj \<and> obj \<in> objs (add' ! i)))
-            \<and> (\<forall>i < length del. \<forall>v \<in> sf_free_vars (del ! i). (\<exists>obj. f (term.VAR v) = inst_term.OBJ obj \<and> obj \<in> objs (del' ! i)))"
-  proof -
-    have well_inst:
-     "\<forall>v \<in> sf_free_vars \<phi>. (\<exists>obj. f (term.VAR v) = inst_term.OBJ obj \<and> obj \<in> objs (cap_avoid_map f \<phi>))"
-      if "wf_fmla upd_te (ty_term (map_of params) constT) \<phi>"
-        for \<phi> 
-    proof -
-      from that 
-      have  "sf_free_vars \<phi> \<subseteq> dom (map_of params)" 
-        using wf_schematic_fmla_free_vars[of "map_of params"]
-        by force
-      hence "sf_free_vars \<phi> \<subseteq> set (map fst params)"
-        by (simp add: dom_map_of_conv_image_fst)
-      moreover
-      from match
-      have "length params = length args"
-        unfolding action_params_match_def using list_all2_lengthD by fastforce
-      hence "length (map fst params) = length (map inst_term.OBJ args)"
-        by fastforce
-      hence "\<forall>v \<in> set (map fst params).(\<exists>obj. (map_of (zip (map fst params) (map inst_term.OBJ args))) v = Some (inst_term.OBJ obj))"
-        find_theorems name: "map_of_zip"
-        apply -
-        apply (rule ballI)
-        subgoal for v
-          apply (drule map_of_zip_is_Some)
-          apply auto[1]
-          apply (drule map_of_SomeD)
-          apply (erule in_set_zipE)
-          by auto
-        done
-      ultimately
-      have "\<forall>v \<in> sf_free_vars \<phi>.(\<exists>obj. (the o (map_of (zip (map fst params) (map inst_term.OBJ args)))) v = inst_term.OBJ obj)"
-        by fastforce
-      hence "\<forall>v \<in> sf_free_vars \<phi>.(\<exists>obj. f (term.VAR v) = inst_term.OBJ obj)"
-        by simp
-      moreover
-      have 2: "\<forall>c. f (term.CONST c) = inst_term.OBJ c" by simp
-      ultimately
-      show "\<forall>v \<in> sf_free_vars \<phi>. (\<exists>obj. f (term.VAR v) = inst_term.OBJ obj \<and> obj \<in> objs (cap_avoid_map f \<phi>))"
-        using cam_instantiates_fv_to_obj by blast
-    qed
-
-    have "\<forall>v \<in> sf_free_vars pre. (\<exists>obj. f (term.VAR v) = inst_term.OBJ obj \<and> obj \<in> objs (cap_avoid_map f pre))" 
-      using wf well_inst by (auto simp: Let_def)
-    hence "\<forall>v \<in> sf_free_vars pre. (\<exists>obj. f (term.VAR v) = inst_term.OBJ obj \<and> obj \<in> objs pre')"
-      using inst by (auto simp: Let_def)
-    moreover
-    have "\<forall>v \<in> sf_free_vars (add ! i). (\<exists>obj. f (term.VAR v) = inst_term.OBJ obj \<and> obj \<in> objs (add' ! i))"
-      if "i < length add" for i
-    proof -
-      have "wf_fmla_atom (ty_term (map_of params) constT) (add ! i)" 
-        using wf that by (auto simp: Let_def)
-      hence "wf_fmla upd_te (ty_term (map_of params) constT) (add ! i)" 
-        using wf_fmla_atom_alt by blast
-      moreover have "add' ! i = cap_avoid_map f (add ! i)" using inst that by (auto simp: Let_def)
-      ultimately show "\<forall>v \<in> sf_free_vars (add ! i). (\<exists>obj. f (term.VAR v) = inst_term.OBJ obj \<and> obj \<in> objs (add' ! i))"
-        using well_inst by auto
-    qed
-    moreover
-    have "\<forall>v \<in> sf_free_vars (del ! i). (\<exists>obj. f (term.VAR v) = inst_term.OBJ obj \<and> obj \<in> objs (del' ! i))"
-      if "i < length del" for i
-    proof -
-      have "wf_fmla_atom (ty_term (map_of params) constT) (del ! i)" 
-        using wf that by (auto simp: Let_def)
-      hence "wf_fmla upd_te (ty_term (map_of params) constT) (del ! i)" 
-        using wf_fmla_atom_alt by blast
-      moreover have "del' ! i = cap_avoid_map f (del ! i)" using inst that by (auto simp: Let_def)
-      ultimately 
-      show "\<forall>v \<in> sf_free_vars (del ! i). (\<exists>obj. f (term.VAR v) = inst_term.OBJ obj \<and> obj \<in> objs (del' ! i))"
-        using well_inst by auto
-    qed
-    ultimately 
-    show ?thesis by fastforce
-  qed
-
 end \<comment> \<open>Context of \<open>ast_problem\<close>\<close>
-
-
 
 subsubsection \<open>Preservation\<close>
 
@@ -2157,7 +1265,7 @@ context ast_problem begin
     \<and> plan_action_path (execute_plan_action \<pi> M) \<pi>s M'"
     by (auto
       simp: plan_action_path_def execute_plan_action_def
-            execute_inst_action_def plan_action_enabled_def)
+            execute_ground_action_def plan_action_enabled_def)
 
 
 
@@ -2174,7 +1282,7 @@ context wf_ast_problem begin
   text \<open>Application of a well-formed effect preserves well-formedness
     of the model\<close>
   lemma wf_apply_effect:
-    assumes "wf_effect (ty_inst_term (\<lambda>_.None) objT) e"
+    assumes "wf_effect objT e"
     assumes "wf_world_model s"
     shows "wf_world_model (apply_effect e s)"
     using assms wf_problem
@@ -2206,12 +1314,12 @@ context wf_ast_problem begin
       unfolding resolve_action_schema_def by auto
     with wf_domain have "wf_action_schema a"
       unfolding wf_domain_def by auto
-    hence "wf_inst_action (resolve_instantiate \<pi>)"
+    hence "wf_ground_action (resolve_instantiate \<pi>)"
       using \<open>resolve_action_schema name = Some a\<close> T
         wf_instantiate_action_schema
       by auto
     thus ?thesis
-      apply (simp add: execute_plan_action_def execute_inst_action_def)
+      apply (simp add: execute_plan_action_def execute_ground_action_def)
       apply (rule wf_apply_effect)
       apply (cases "resolve_instantiate \<pi>"; simp)
       by (rule \<open>wf_world_model s\<close>)
